lib/Marshalling/MarshalledAccessors.i.dfy
@@ -6,6 +6,7 @@ include "../Base/mathematics.i.dfy"
 include "../Base/sequences.i.dfy"
 include "Math.i.dfy"
 include "NLarith.i.dfy"
+include "../Base/Slice.i.dfy"
 
 /////////////////////////////////////////
 // The most general marshalling interface
@@ -14,86 +15,94 @@ include "NLarith.i.dfy"
 abstract module Marshalling {
   import opened NativeTypes
   import opened Options
+  import opened Slices
 
   type UnmarshalledType
 
-  // "mseq" == "machine seq"
-  type mseq<T> = s : seq<T> | |s| < Uint64UpperBound()
+  type Config
 
-  predicate parsable(data: mseq<byte>)
+  predicate validConfig(cfg: Config)
 
-  function parse(data: mseq<byte>) : UnmarshalledType
-    requires parsable(data)
+  predicate parsable(cfg: Config, data: mseq<byte>)
+    requires validConfig(cfg)
 
-  method TryParse(data: mseq<byte>) returns (ovalue: Option<UnmarshalledType>)
-    ensures parsable(data) <==> ovalue.Some?
-    ensures parsable(data) ==> ovalue.value == parse(data)
+  function parse(cfg: Config, data: mseq<byte>) : UnmarshalledType
+    requires validConfig(cfg)
+    requires parsable(cfg, data)
 
-  // FIXME: robj: Would like to provide this as default implementations,
-  // but overriding in in refining modules gives an error about
-  // assigning to p.
-  method Parsable(data: mseq<byte>) returns (p: bool)
-    ensures p == parsable(data)
-  // {
-  //   var ovalue := TryParse(data);
-  //   p := ovalue.Some?;
-  // }
+  method TryParse(cfg: Config, data: mseq<byte>) returns (ovalue: Option<UnmarshalledType>)
+    requires validConfig(cfg)
+    ensures parsable(cfg, data) <==> ovalue.Some?
+    ensures parsable(cfg, data) ==> ovalue.value == parse(cfg, data)
 
-  // FIXME: robj: Would like to provide this as default
-  // implementations, but overriding in in refining modules gives an
-  // error about assigning to p.
-  method Parse(data: mseq<byte>) returns (value: UnmarshalledType)
-    requires parsable(data)
-    ensures value == parse(data)
-  // {
-  //   var ovalue := TryParse(data);
-  //   value := ovalue.value;
-  // }
+  method Parsable(cfg: Config, data: mseq<byte>) returns (p: bool)
+    requires validConfig(cfg)
+    ensures p == parsable(cfg, data)
+  {
+    var ovalue := TryParse(cfg, data);
+    p := ovalue.Some?;
+  }
 
-  predicate marshallable(value: UnmarshalledType)
+  method Parse(cfg: Config, data: mseq<byte>) returns (value: UnmarshalledType)
+    requires validConfig(cfg)
+    requires parsable(cfg, data)
+    ensures value == parse(cfg, data)
+  {
+    var ovalue := TryParse(cfg, data);
+    value := ovalue.value;
+  }
 
-  function size(value: UnmarshalledType) : nat
-    requires marshallable(value)
+  predicate marshallable(cfg: Config, value: UnmarshalledType)
+    requires validConfig(cfg)
 
-  method Size(value: UnmarshalledType) returns (sz: uint64)
-    requires marshallable(value)
-    requires size(value) < Uint64UpperBound()
-    ensures sz as nat == size(value)
+  function size(cfg: Config, value: UnmarshalledType) : uint64
+    requires validConfig(cfg)
+    requires marshallable(cfg, value)
 
-  // FIXME: robj: data should be linear inout doesn't work with module
-  // refinement.
-  method Marshall(value: UnmarshalledType, linear data: mseq<byte>, start: uint64)
-    returns (linear newdata: mseq<byte>, end: uint64)
-    requires marshallable(value)
-    requires start as nat + size(value) <= |data|
-    ensures end as nat == start as nat + size(value)
-    ensures |newdata| == |data|
-    ensures forall i | 0 <= i < start :: newdata[i] == data[i]
-    ensures forall i | end <= i < |newdata| as uint64 :: newdata[i] == data[i]
-    ensures parsable(newdata[start..end])
-    ensures parse(newdata[start..end]) == value
+  method Size(cfg: Config, value: UnmarshalledType) returns (sz: uint64)
+    requires validConfig(cfg)
+    requires marshallable(cfg, value)
+    ensures sz == size(cfg, value)
+
+  method Marshall(cfg: Config, value: UnmarshalledType, linear inout data: mseq<byte>, start: uint64)
+    returns (end: uint64)
+    requires validConfig(cfg)
+    requires marshallable(cfg, value)
+    requires start as nat + size(cfg, value) as nat <= |old_data|
+    ensures end == start + size(cfg, value)
+    ensures |data| == |old_data|
+    ensures forall i | 0 <= i < start :: data[i] == old_data[i]
+    ensures forall i | end <= i < |data| as uint64 :: data[i] == old_data[i]
+    ensures parsable(cfg, data[start..end])
+    ensures parse(cfg, data[start..end]) == value
 }
 
 ////////////////////////////////////////////////////
 // Marshalling implementation for a packable integer
 ////////////////////////////////////////////////////
 
-abstract module IntegerMarshalling(Int: NativePackedInt) refines Marshalling {
+module IntegerMarshalling(Int: NativePackedInt) refines Marshalling {
   import opened LinearSequence_s
 
   type UnmarshalledType = Int.Integer
 
-  predicate parsable(data: mseq<byte>)
+  datatype Config = DefaultConfig
+
+  predicate validConfig(cfg: Config) {
+    true
+  }
+
+  predicate parsable(cfg: Config, data: mseq<byte>)
   {
     Int.Size() as nat <= |data|
   }
 
-  function parse(data: mseq<byte>) : UnmarshalledType
+  function parse(cfg: Config, data: mseq<byte>) : UnmarshalledType
   {
     Int.unpack(data[..Int.Size()])
   }
 
-  method TryParse(data: mseq<byte>) returns (ovalue: Option<UnmarshalledType>)
+  method TryParse(cfg: Config, data: mseq<byte>) returns (ovalue: Option<UnmarshalledType>)
   {
     if Int.Size() <= |data| as uint64 {
       var value := Int.Cast(data, 0);
@@ -103,37 +112,38 @@ abstract module IntegerMarshalling(Int: NativePackedInt) refines Marshalling {
     }
   }
 
-  method Parsable(data: mseq<byte>) returns (p: bool)
+  method Parsable(cfg: Config, data: mseq<byte>) returns (p: bool)
   {
-    p := Int.Size() <= |data| as uint64;
+    var p' := Int.Size() <= |data| as uint64;
+    return p';
   }
 
-  method Parse(data: mseq<byte>) returns (value: UnmarshalledType)
+  method Parse(cfg: Config, data: mseq<byte>) returns (value: UnmarshalledType)
   {
-    value := Int.Cast(data, 0);
+    var value' := Int.Cast(data, 0);
+    return value';
   }
 
-  predicate marshallable(value: UnmarshalledType) {
+  predicate marshallable(cfg: Config, value: UnmarshalledType) {
     true
   }
 
-  function size(value: UnmarshalledType) : nat
+  function size(cfg: Config, value: UnmarshalledType) : uint64
   {
-    Int.Size() as nat
+    Int.Size()
   }
 
-  method Size(value: UnmarshalledType) returns (sz: uint64)
+  method Size(cfg: Config, value: UnmarshalledType) returns (sz: uint64)
   {
     sz := Int.Size();
   }
 
-  method Marshall(value: UnmarshalledType, linear data: mseq<byte>, start: uint64)
-    returns (linear newdata: mseq<byte>, end: uint64)
+  method Marshall(cfg: Config, value: UnmarshalledType, linear inout data: mseq<byte>, start: uint64)
+    returns (end: uint64)
   {
-      newdata := data;
-      Int.Pack_into_ByteSeq(value, inout newdata, start);
+      Int.Pack_into_ByteSeq(value, inout data, start);
       end := start + Int.Size();
-      assert newdata[start..end][..Int.Size()] == newdata[start..start + Int.Size()];
+      assert data[start..end][..Int.Size()] == data[start..start + Int.Size()];
   }
 }
 
@@ -145,452 +155,245 @@ module Uint64Marshalling refines IntegerMarshalling(NativePackedUint64) {
 
 //////////////////////////////////////////////////////////////////////
 // Interface for marshalling sequences
-//
-// This adds support for querying the length of the sequence and
-// getting the marshalled representation of an element of the sequence
-// without having to parse the whole thing.
 //////////////////////////////////////////////////////////////////////
 
-abstract module SeqMarshalling(ElementMarshalling: Marshalling) refines Marshalling {
-  type Element = ElementMarshalling.UnmarshalledType
+abstract module SeqMarshalling(Elt: Marshalling) refines Marshalling {
+  import opened LinearSequence_s
+  import opened LinearSequence_i
+
+  type Element = Elt.UnmarshalledType
   type UnmarshalledType = mseq<Element>
 
-  predicate lengthable(data: mseq<byte>)
-    ensures parsable(data) ==> lengthable(data)
+  function method EltCfg(cfg: Config) : Elt.Config
+    requires validConfig(cfg)
+    ensures Elt.validConfig(EltCfg(cfg))
 
-  method TryLength(data: mseq<byte>) returns (olen: Option<uint64>)
-    ensures lengthable(data) <==> olen.Some?
-    ensures parsable(data) ==> olen.value as nat == |parse(data)|
+    // lengths
+  predicate lengthable(cfg: Config, data: mseq<byte>)
+    requires validConfig(cfg)
 
-  method Lengthable(data: mseq<byte>) returns (l: bool)
-    ensures l == lengthable(data)
+  function length(cfg: Config, data: mseq<byte>) : nat
+    requires validConfig(cfg)
+    requires lengthable(cfg, data)
 
-  method Length(data: mseq<byte>) returns (len: uint64)
-    requires lengthable(data)
-    ensures parsable(data) ==> len as nat == |parse(data)|
+  method TryLength(cfg: Config, data: mseq<byte>) returns (olen: Option<uint64>)
+    requires validConfig(cfg)
+    ensures olen.Some? <==> lengthable(cfg, data)
+    ensures olen.Some? ==> olen.value as nat == length(cfg, data)
 
+  method Lengthable(cfg: Config, data: mseq<byte>) returns (l: bool)
+    requires validConfig(cfg)
+    ensures l == lengthable(cfg, data)
 
-  predicate gettable(data: mseq<byte>, idx: nat)
-    ensures parsable(data) && idx < |parse(data)| ==> gettable(data, idx)
-
-  method TryGet(data: mseq<byte>, idx: uint64) returns (oedata: Option<mseq<byte>>)
-    ensures oedata.Some? <==> gettable(data, idx as nat)
-    ensures parsable(data) && |parse(data)| <= idx as nat ==> oedata.None?
-    ensures parsable(data) && idx as nat < |parse(data)| ==> ElementMarshalling.parsable(oedata.value)
-    ensures parsable(data) && idx as nat < |parse(data)| ==> ElementMarshalling.parse(oedata.value) == parse(data)[idx]
-
-  method Gettable(data: mseq<byte>, idx: uint64) returns (g: bool)
-    ensures g == gettable(data, idx as nat)
+  method Length(cfg: Config, data: mseq<byte>) returns (len: uint64)
+    requires validConfig(cfg)
+    requires lengthable(cfg, data)
+    ensures len as nat == length(cfg, data)
 
 
-  method Get(data: mseq<byte>, idx: uint64) returns (edata: mseq<byte>)
-    requires gettable(data, idx as nat)
-    ensures parsable(data) && idx as nat < |parse(data)| ==> ElementMarshalling.parsable(edata)
-    ensures parsable(data) && idx as nat < |parse(data)| ==> ElementMarshalling.parse(edata) == parse(data)[idx]
-}
+    // getting individual elements
+  predicate gettable(cfg: Config, data: mseq<byte>, idx: nat)
+    requires validConfig(cfg)
 
-//////////////////////////////////////////////////////////////////////
-// Common parts of implementation of marshalling a sequence of items
-// that all have the same marshalled size.
-//
-// We omit the actual parsing and marshalling implementations so that
-// we can use the optimized integer packing code.
-//////////////////////////////////////////////////////////////////////
+  function get(cfg: Config, slice: Slice, data: mseq<byte>, idx: nat) : (eslice: Slice)
+    requires validConfig(cfg)
+    requires slice.WF'(data)
+    requires gettable(cfg, slice.I(data), idx)
+    ensures eslice.WF'(data)
 
-abstract module UniformSizedElementSeqMarshallingCommon(elementMarshalling: Marshalling)
-refines SeqMarshalling(elementMarshalling) {
-  import opened Mathematics
-  import opened LinearSequence_i
-  import opened LinearSequence_s
-  import Seq = Sequences
-  import opened Math
-  import NLarith
-
-  function method UniformSize() : uint64
-    ensures 0 < UniformSize()
-
-  predicate lengthable(data: mseq<byte>)
+  function getData(cfg: Config, data: mseq<byte>, idx: nat) : (edata: mseq<byte>)
+    requires validConfig(cfg)
+    requires gettable(cfg, data, idx)
   {
-    true
+    get(cfg, all(data), data, idx).I(data)
   }
 
-  function length(data: mseq<byte>) : nat
-    ensures length(data) <=  length(data) * UniformSize() as nat <= |data|
+  function getElt(cfg: Config, data: mseq<byte>, idx: nat) : (elt: Element)
+    requires validConfig(cfg)
+    requires gettable(cfg, data, idx)
+    requires Elt.parsable(EltCfg(cfg), getData(cfg, data, idx))
   {
-    NLarith.DivLe(|data|, UniformSize() as nat);
-    DivMulOrder(|data|, UniformSize() as nat);
-    assert (|data| / UniformSize() as nat) * 1 == |data| / UniformSize() as nat;
-    if 1 < UniformSize() then
-      PosMulPreservesOrder(1, UniformSize() as nat, |data| / UniformSize() as nat);
-      |data| / UniformSize() as nat
-    else 
-      |data| / UniformSize() as nat
+    Elt.parse(EltCfg(cfg), getData(cfg, data, idx))
   }
 
-  method TryLength(data: mseq<byte>) returns (olen: Option<uint64>)
-  {
-    NLarith.DivLe(|data|, UniformSize() as nat);
-    olen := Some(|data| as uint64 / UniformSize());
-  }
+  method TryGet(cfg: Config, slice: Slice, data: mseq<byte>, idx: uint64) returns (oeslice: Option<Slice>)
+    requires validConfig(cfg)
+    requires slice.WF'(data)
+    ensures oeslice.Some? <==> gettable(cfg, slice.I(data), idx as nat)
+    ensures oeslice.Some? ==> oeslice.value == get(cfg, slice, data, idx as nat)
 
-  method Lengthable(data: mseq<byte>) returns (l: bool)
-  {
-    l := true;
-  }
+  method Gettable(cfg: Config, data: mseq<byte>, idx: uint64) returns (g: bool)
+    requires validConfig(cfg)
+    ensures g == gettable(cfg, data, idx as nat)
 
-  method Length(data: mseq<byte>) returns (len: uint64)
-    ensures len as nat == length(data)
-  {
-    NLarith.DivLe(|data|, UniformSize() as nat);
-    len := |data| as uint64 / UniformSize();
-  }
 
-  lemma index_bounds_facts(data: mseq<byte>, idx: nat)
-    requires idx < length(data)
-    ensures 0 <= idx * UniformSize() as nat < idx * UniformSize() as nat + UniformSize() as nat == (idx + 1) * UniformSize() as nat <= |data|
+  method Get(cfg: Config, slice: Slice, data: mseq<byte>, idx: uint64) returns (eslice: Slice)
+    requires validConfig(cfg)
+    requires slice.WF'(data)
+    requires gettable(cfg, slice.I(data), idx as nat)
+    ensures eslice.WF()
+    ensures eslice == get(cfg, slice, data, idx as nat)
+
+  method TryGetParsed(cfg: Config, data: mseq<byte>, idx: uint64) returns (oelt: Option<Element>)
+    requires validConfig(cfg)
+    ensures oelt.Some? <==> gettable(cfg, data, idx as nat) && Elt.parsable(EltCfg(cfg), getData(cfg, data, idx as nat))
+    ensures oelt.Some? ==> oelt.value == getElt(cfg, data, idx as nat)
   {
-    NatMulNatIsNat(idx, UniformSize() as nat);
-    PosMulPreservesOrder(idx, idx + 1, UniformSize() as nat);
-    NLarith.DistributeLeft(idx, 1, UniformSize() as nat);
-    if idx + 1 < length(data) {
-      PosMulPreservesOrder(idx + 1, length(data), UniformSize() as nat);
+    var oeslice := TryGet(cfg, all(data), data, idx);
+    if oeslice == None {
+      return None;
     }
+    oelt := Elt.TryParse(EltCfg(cfg), oeslice.value.I(data));
   }
 
-  function method ElementData(data: mseq<byte>, idx: uint64) : mseq<byte>
-    requires idx as nat < length(data)
-    ensures |ElementData(data, idx)| == UniformSize() as nat
+  method GetParsed(cfg: Config, data: mseq<byte>, idx: uint64) returns (elt: Element)
+    requires validConfig(cfg)
+    requires gettable(cfg, data, idx as nat)
+    requires Elt.parsable(EltCfg(cfg), getData(cfg, data, idx as nat))
+    ensures elt == getElt(cfg, data, idx as nat)
   {
-    index_bounds_facts(data, idx as nat);
-    data[idx * UniformSize()..idx * UniformSize() + UniformSize()]
+    var eslice := Get(cfg, all(data), data, idx);
+    elt := Elt.Parse(EltCfg(cfg), eslice.I(data));
   }
 
-  predicate parsable(data: mseq<byte>) {
-    forall idx | 0 <= idx < length(data) :: elementMarshalling.parsable(ElementData(data, idx as uint64))
-  }
+    // setting individual elements
+  predicate settable(cfg: Config, data: mseq<byte>, idx: nat, value: Element)
+    requires validConfig(cfg)
+    requires Elt.marshallable(EltCfg(cfg), value)
 
-  function parse_prefix(data: mseq<byte>, len: nat) : (result: UnmarshalledType)
-    requires parsable(data)
-    requires len <= length(data)
-    ensures |result| == len
-    ensures forall i | 0 <= i < len :: result[i] == elementMarshalling.parse(ElementData(data, i as uint64))
+  predicate preservesEntry(cfg: Config, data: mseq<byte>, i: nat, newdata: mseq<byte>)
+    requires validConfig(cfg)
   {
-    if len == 0 then
-      []
-    else
-      var prefix := parse_prefix(data, len - 1);
-      var last := elementMarshalling.parse(ElementData(data, len as uint64 - 1));
-      prefix + [last]
+    && (gettable(cfg, data, i) ==> gettable(cfg, newdata, i))
+    && ((gettable(cfg, data, i) && Elt.parsable(EltCfg(cfg), getData(cfg, data, i))) ==>
+       (Elt.parsable(EltCfg(cfg), getData(cfg, newdata, i)) && getElt(cfg, newdata, i) == getElt(cfg, data, i)))
   }
 
-  function parse(data: mseq<byte>) : (result: UnmarshalledType)
+  predicate sets(cfg: Config, data: mseq<byte>, idx: nat, value: Element, newdata: mseq<byte>)
+    requires validConfig(cfg)
+    requires Elt.marshallable(EltCfg(cfg), value)
+    requires settable(cfg, data, idx, value)
   {
-    var len := length(data);
-    parse_prefix(data, len)
-  }
-
-  predicate gettable(data: mseq<byte>, idx: nat)
-  {
-    idx < length(data)
-  }
-
-  method TryGet(data: mseq<byte>, idx: uint64) returns (oedata: Option<mseq<byte>>)
-  {
-    var len := Length(data);
-    if idx < len {
-      oedata := Some(ElementData(data, idx));
-    } else {
-      oedata := None;
-    }
-  }
-
-  method Gettable(data: mseq<byte>, idx: uint64) returns (g: bool)
-  {
-    var len := Length(data);
-    g := idx < len;
-  }
-
-  method Get(data: mseq<byte>, idx: uint64) returns (edata: mseq<byte>)
-  {
-    edata := ElementData(data, idx);
-  }
-
-
-  predicate marshallable(value: UnmarshalledType)
-  {
-    && (forall i | 0 <= i < |value| :: elementMarshalling.marshallable(value[i]))
-    && (forall i | 0 <= i < |value| :: elementMarshalling.size(value[i]) == UniformSize() as nat)
-  }
-
-  lemma marshallable_prefix(value: UnmarshalledType, len: nat)
-    requires marshallable(value)
-    requires 0 <= len <= |value|
-    ensures marshallable(value[..len])
-  {
-  }
-
-  function size(value: UnmarshalledType) : nat
-  {
-    NatMulNatIsNat(|value|, UniformSize() as nat);
-    |value| * UniformSize() as nat
-  }
-
-  method Size(value: UnmarshalledType) returns (sz: uint64)
-  {
-    sz := |value| as uint64 * UniformSize();
-  }
-
-  lemma parsing_extend(data: mseq<byte>, edata: mseq<byte>)
-    requires parsable(data)
-    requires |data| == length(data) * UniformSize() as nat
-    requires elementMarshalling.parsable(edata)
-    requires |edata| == UniformSize() as nat
-    requires |data + edata| < Uint64UpperBound()
-    ensures parsable(data + edata)
-    ensures parse(data + edata) == parse(data) + [ elementMarshalling.parse(edata) ]
-  {
-    var extension := data + edata;
-    lemma_div_ind(|data|, UniformSize() as nat);
-    forall idx | 0 <= idx < length(data)
-      ensures ElementData(extension, idx as uint64) == ElementData(data, idx as uint64);
-    {
-      index_bounds_facts(data, idx);
-      Seq.lemma_seq_slice_slice(extension, 0, |data|, idx * UniformSize() as nat, idx * UniformSize() as nat + UniformSize() as nat);
-    }
-    assert ElementData(extension, length(data) as uint64) == edata;
-    assert parse(extension)[..length(data)] == parse(data);
-  }
-
-  predicate settable(data: mseq<byte>, idx: nat, value: Element) {
-    && idx < length(data)
-    && elementMarshalling.marshallable(value)
-    && elementMarshalling.size(value) == UniformSize() as nat
-  }
-
-  method Settable(data: mseq<byte>, idx: uint64, value: Element) returns (s: bool)
-    requires elementMarshalling.marshallable(value)
-    requires elementMarshalling.size(value) < Uint64UpperBound()
-    ensures s == settable(data, idx as nat, value)
-  {
-    var len := Length(data);
-    var sz := elementMarshalling.Size(value);
-    return idx < len && sz == UniformSize();
-  }
-
-  predicate setted(data: mseq<byte>, idx: nat, value: Element, newdata: mseq<byte>)
-    requires settable(data, idx, value)
-  {
-    index_bounds_facts(data, idx);
     && |newdata| == |data|
-    && (forall i | 0 <= i < idx * UniformSize() as nat :: newdata[i] == data[i])
-    && (forall i | (idx+1) * UniformSize() as nat <= i < |data| :: newdata[i] == data[i])
-    && elementMarshalling.parsable(newdata[idx * UniformSize() as nat..(idx+1) * UniformSize() as nat])
-    && elementMarshalling.parse(newdata[idx * UniformSize() as nat..(idx+1) * UniformSize() as nat]) == value
+    && (lengthable(cfg, data) ==> lengthable(cfg, newdata) && length(cfg, newdata) == length(cfg, data))
+    && (forall i | i != idx :: preservesEntry(cfg, data, i, newdata))
+    && gettable(cfg, newdata, idx)
+    && Elt.parsable(EltCfg(cfg), getData(cfg, newdata, idx))
+    && getElt(cfg, newdata, idx) == value
   }
 
-  lemma setted_parsing(data: mseq<byte>, idx: nat, value: Element, newdata: mseq<byte>)
-    requires parsable(data)
-    requires settable(data, idx, value)
-    requires setted(data, idx, value, newdata)
-    ensures lengthable(newdata)
-    ensures length(newdata) == length(data)
-    ensures parsable(newdata)
-    ensures |parse(newdata)| == |parse(data)|
-    ensures idx as nat < |parse(data)|
-    ensures parse(newdata) == parse(data)[idx as nat := value]
-  {
-    assert length(newdata) == length(data);
+  method Settable(cfg: Config, data: mseq<byte>, idx: uint64, value: Element) returns (s: bool)
+    requires validConfig(cfg)
+    requires Elt.marshallable(EltCfg(cfg), value)
+    ensures s == settable(cfg, data, idx as nat, value)
 
-    forall i | 0 <= i < length(newdata)
-      ensures elementMarshalling.parsable(ElementData(newdata, i as uint64))
-      ensures elementMarshalling.parse(ElementData(newdata, i as uint64)) == parse(data)[idx as nat := value][i]
-    {
-      index_bounds_facts(data, i);
-      calc {
-        ElementData(newdata, i as uint64);
-        newdata[i * UniformSize() as nat..(i + 1) * UniformSize() as nat];
-        { Seq.lemma_seq_slice_slice(newdata, 0, |data|, i * UniformSize() as nat, (i + 1) * UniformSize() as nat); }
-        newdata[i * UniformSize() as nat..(i + 1) * UniformSize() as nat];
-      }
-      calc {
-        ElementData(data, i as uint64);
-        data[i * UniformSize() as nat..(i + 1) * UniformSize() as nat];
-        { Seq.lemma_seq_slice_slice(data, 0, |data|, i * UniformSize() as nat, (i + 1) * UniformSize() as nat); }
-        data[i * UniformSize() as nat..(i + 1) * UniformSize() as nat];
-      }
-      if i == idx as nat {
-        assert elementMarshalling.parsable(ElementData(newdata, i as uint64));
-      } else {
-        forall j: nat | i * UniformSize() as nat <= j < (i+1) * UniformSize() as nat
-          ensures j < |newdata|
-          ensures newdata[j] == data[j]
-          {
-            if i < idx as nat {
-              assert i + 1 <= idx;
-              if i + 1 < idx {
-                PosMulPreservesOrder(i + 1, idx, UniformSize() as nat);
-              }
-            } else {
-              assert idx + 1 <= i;
-              if idx + 1 < i {
-                PosMulPreservesOrder(idx + 1, i, UniformSize() as nat);
-              }
-            }
-          }
-          Seq.lemma_seq_extensionality_slice(data, newdata, i * UniformSize() as nat, (i+1) * UniformSize() as nat);
-      }
+  method Set(cfg: Config, slice: Slice, linear inout data: mseq<byte>, idx: uint64, value: Element)
+    requires validConfig(cfg)
+    requires slice.WF'(old_data)
+    requires Elt.marshallable(EltCfg(cfg), value)
+    requires settable(cfg, slice.I(old_data), idx as nat, value)
+    ensures |data| == |old_data|
+    ensures forall i | 0 <= i < slice.start :: data[i] == old_data[i]
+    ensures forall i | slice.end <= i < |data| as uint64 :: data[i] == old_data[i]
+    ensures sets(cfg, slice.I(old_data), idx as nat, value, slice.I(data))
+
+
+    // resizing
+  predicate resizable(cfg: Config, data: mseq<byte>, newlen: nat)
+    requires validConfig(cfg)
+
+  predicate resizes(cfg: Config, data: mseq<byte>, newlen: nat, newdata: mseq<byte>)
+    requires validConfig(cfg)
+    requires resizable(cfg, data, newlen)
+  {
+    && |newdata| == |data|
+    && lengthable(cfg, newdata)
+    && length(cfg, newdata) == newlen
+    && (forall i :: preservesEntry(cfg, data, i, newdata))
+  }
+
+  method Resizable(cfg: Config, data: mseq<byte>, newlen: uint64) returns (r: bool)
+    requires validConfig(cfg)
+    ensures r == resizable(cfg, data, newlen as nat)
+
+  method Resize(cfg: Config, slice: Slice, linear inout data: mseq<byte>, newlen: uint64)
+    requires validConfig(cfg)
+    requires slice.WF'(old_data)
+    requires resizable(cfg, slice.I(old_data), newlen as nat)
+    ensures |data| == |old_data|
+    ensures forall i | 0 <= i < slice.start :: data[i] == old_data[i]
+    ensures forall i | slice.end <= i < |data| as uint64 :: data[i] == old_data[i]
+    ensures resizes(cfg, slice.I(old_data), newlen as nat, slice.I(data))
+
+
+    // append
+  predicate appendable(cfg: Config, data: mseq<byte>, value: Element)
+    requires validConfig(cfg)
+    ensures lengthable(cfg, data)
+
+  predicate appends(cfg: Config, data: mseq<byte>, value: Element, newdata: mseq<byte>)
+    requires validConfig(cfg)
+    requires appendable(cfg, data, value)
+  {
+    var oldlen := length(cfg, data);
+    && |newdata| == |data|
+    && lengthable(cfg, newdata)
+    && length(cfg, newdata) == oldlen + 1
+    && (forall i | i != oldlen :: preservesEntry(cfg, data, i, newdata))
+    && gettable(cfg, newdata, oldlen)
+    && Elt.parsable(EltCfg(cfg), getData(cfg, newdata, oldlen))
+    && getElt(cfg, newdata, oldlen) == value
+  }
+
+  method Appendable(cfg: Config, data: mseq<byte>, value: Element) returns (r: bool)
+    requires validConfig(cfg)
+    ensures r == appendable(cfg, data, value)
+
+  method Append(cfg: Config, slice: Slice, linear inout data: mseq<byte>, value: Element)
+    requires validConfig(cfg)
+    requires slice.WF'(old_data)
+    requires appendable(cfg, slice.I(old_data), value)
+    ensures |data| == |old_data|
+    ensures forall i | 0 <= i < slice.start :: data[i] == old_data[i]
+    ensures forall i | slice.end <= i < |data| as uint64 :: data[i] == old_data[i]
+    ensures appends(cfg, slice.I(old_data), value, slice.I(data))
+
+
+  predicate parsableToLen(cfg: Config, data: mseq<byte>, len: uint64)
+    requires validConfig(cfg)
+  {
+    && (forall i | 0 <= i < len :: gettable(cfg, data, i as nat))
+    && (forall i | 0 <= i < len :: Elt.parsable(EltCfg(cfg), getData(cfg, data, i as nat)))
+  }
+
+  predicate parsable(cfg: Config, data: mseq<byte>)
+  {
+    && lengthable(cfg, data)
+    && length(cfg, data) < Uint64UpperBound()
+    && parsableToLen(cfg, data, length(cfg, data) as uint64)
+  }
+
+  function parseToLen(cfg: Config, data: mseq<byte>, len: uint64) : UnmarshalledType
+    requires validConfig(cfg)
+    requires parsableToLen(cfg, data, len)
+  {
+    var r: seq<Element> := seq(len as nat, i requires 0 <= i < len as nat => getElt(cfg, data, i));
+    assert |r| < Uint64UpperBound();
+    r
+  }
+
+  function parse(cfg: Config, data: mseq<byte>) : UnmarshalledType
+  {
+    parseToLen(cfg, data, length(cfg, data) as uint64)
+  }
+
+  method TryParse(cfg: Config, data: mseq<byte>) returns (ovalue: Option<UnmarshalledType>)
+  {
+    var olen := TryLength(cfg, data);
+    if olen == None {
+      return None;
     }
-    assert forall i | 0 <= i < length(newdata) :: parse(newdata)[i] == elementMarshalling.parse(ElementData(newdata, i as uint64));
-  }
-
-  method Set(linear data: mseq<byte>, start: uint64, end: uint64, idx: uint64, value: Element)
-    returns (linear newdata: mseq<byte>)
-    requires start as nat <= end as nat <= |data|
-    requires settable(data[start..end], idx as nat, value)
-    ensures |newdata| == |data|
-    ensures forall i | 0 <= i < start :: newdata[i] == data[i]
-    ensures forall i | end as nat <= i < |newdata| :: newdata[i] == data[i]
-    ensures setted(data[start..end], idx as nat, value, newdata[start..end])
-    ensures lengthable(newdata[start..end])
-    ensures length(newdata[start..end]) == length(data[start..end])
-    ensures parsable(data[start..end]) ==> parsable(newdata[start..end])
-    ensures parsable(data[start..end]) ==> |parse(newdata[start..end])| == |parse(data[start..end])|
-    ensures parsable(data[start..end]) ==> idx as nat < |parse(data[start..end])|
-    ensures parsable(data[start..end]) ==> parse(newdata[start..end]) == parse(data[start..end])[idx as nat := value]
-  {
-    index_bounds_facts(data[start..end], idx as nat);
-
-    var newend;
-    newdata, newend := elementMarshalling.Marshall(value, data, start + idx * UniformSize());
-
-    calc {
-      newdata[start as nat..end][idx as nat * UniformSize() as nat..(idx as nat + 1) * UniformSize() as nat];
-      { Seq.lemma_seq_slice_slice(newdata, start as nat, end as nat, idx as nat * UniformSize() as nat, (idx as nat + 1) * UniformSize() as nat); }
-      newdata[start as nat + idx as nat * UniformSize() as nat..start as nat + (idx as nat + 1) * UniformSize() as nat];
-    }
-    assert setted(data[start..end], idx as nat, value, newdata[start..end]);
-    if parsable(data[start..end]) {
-      setted_parsing(data[start..end], idx as nat, value, newdata[start..end]);
-    }
-  }
-}
-
-
-/////////////////////////////////////////////////////////////////
-// Implementation for marshalling a sequence of packable integers
-//
-// We could just use the UniformSized marshalling code further below,
-// but that would marshall each integer one at a time, which would
-// (presumably) be slower.
-/////////////////////////////////////////////////////////////////
-
-abstract module IntegerSeqMarshalling(Int: NativePackedInt)
-refines UniformSizedElementSeqMarshallingCommon(IntegerMarshalling(Int)) {
-  function method UniformSize() : uint64 {
-    Int.Size()
-  }
-
-  lemma always_parsable(data: mseq<byte>)
-    ensures parsable(data)
-  {
-    var len := length(data);
-    forall i | 0 <= i < len
-      ensures elementMarshalling.parsable(ElementData(data, i as uint64))
-    {
-      DivMulOrder(length(data), UniformSize() as nat);
-      assert i + 1 <= length(data);
-      if i + 1 < length(data) {
-        PosMulPreservesOrder(i + 1, length(data), UniformSize() as nat);
-      }
-      assert (i + 1) * UniformSize() as nat <=  length(data) * UniformSize() as nat;
-      assert length(data) * UniformSize() as nat <= |data|;
-      assert (i + 1) * UniformSize() as nat <= |data|;
-    }
-  }
-
-  lemma parse_is_unpack_Seq(data: mseq<byte>)
-    requires parsable(data)
-    ensures parse(data) == Int.unpack_Seq(data[..length(data) * Int.Size() as nat], length(data))
-  {
-    var len := length(data);
-    var value := Int.unpack_Seq(data[..len * Int.Size() as nat], len);
-    forall i | 0 <= i < |value|
-      ensures value[i] == parse(data)[i]
-    {
-      index_bounds_facts(data, i);
-      if i + 1 < len {
-        PosMulPreservesOrder(i + 1, len, Int.Size() as nat);
-      }
-      Seq.lemma_seq_slice_slice(data, 0, Int.Size() as nat * len as nat, i * Int.Size() as nat, (i+1) * Int.Size() as nat);
-      Seq.lemma_seq_slice_slice(data, i * UniformSize() as nat, (i + 1) * UniformSize() as nat, 0, Int.Size() as nat);
-    }
-  }
-
-  method TryParse(data: mseq<byte>) returns (ovalue: Option<UnmarshalledType>)
-  {
-    var len := Length(data);
-    var value := Int.Cast_Seq(data, 0, len);
-    assert |value| < Uint64UpperBound();
-    ovalue := Some(value);
-    always_parsable(data);
-    parse_is_unpack_Seq(data);
-  }
-
-  method Parsable(data: mseq<byte>) returns (p: bool)
-  {
-    always_parsable(data);
-    p := true;
-  }
-
-  method Parse(data: mseq<byte>) returns (value: UnmarshalledType)
-  {
-    var length := Length(data);
-    value := Int.Cast_Seq(data, 0, length);
-    parse_is_unpack_Seq(data);
-  }
-
-  method FastGet(data: mseq<byte>, idx: uint64) returns (element: Element)
-    requires idx as nat < length(data)
-    ensures parsable(data);
-    ensures element == parse(data)[idx]
-  {
-    index_bounds_facts(data, idx as nat);
-    always_parsable(data);
-    element := Int.Cast(data, idx * Int.Size());
-    assert data[idx * Int.Size()..idx * Int.Size() + Int.Size()] == data[idx * Int.Size()..idx * Int.Size() + Int.Size()][..Int.Size()];
-  }
-
-  method Marshall(value: UnmarshalledType, linear data: mseq<byte>, start: uint64)
-    returns (linear newdata: mseq<byte>, end: uint64)
-  {
-    newdata := data;
-    Int.Pack_Seq_into_ByteSeq(value, inout newdata, start);
-    var sz := Size(value);
-    end := start + sz;
-
-    always_parsable(newdata[start..end]);
-    parse_is_unpack_Seq(newdata[start..end]);
-    MulDivCancel(|value|, Int.Size() as nat);
-    Seq.lemma_seq_slice_slice(newdata, start as nat, end as nat, 0, length(newdata[start..end]) * Int.Size() as nat);
-  }
-}
-
-abstract module Uint32SeqMarshalling refines IntegerSeqMarshalling(NativePackedUint32) {
-}
-
-abstract module Uint64SeqMarshalling refines IntegerSeqMarshalling(NativePackedUint64) {
-}
-
-//////////////////////////////////////////////////////////////////////
-// Implementation of marshalling a sequence of items that all have the
-// same marshalled size.
-//////////////////////////////////////////////////////////////////////
-
-abstract module UniformSizedElementSeqMarshalling(Element_Marshalling: Marshalling)
-refines UniformSizedElementSeqMarshallingCommon(Element_Marshalling) {
-
-  method TryParse(data: mseq<byte>) returns (ovalue: Option<UnmarshalledType>) {
-    var len: uint64 := Length(data);
+    var len := olen.value;
     if len == 0 {
       var empty: UnmarshalledType := [];
       return Some(empty);
@@ -598,7 +401,7 @@ refines UniformSizedElementSeqMarshallingCommon(Element_Marshalling) {
 
     // We get the first element by itself so we can call
     // seq_alloc_init below.
-    var oelt := ElementMarshalling.TryParse(ElementData(data, 0));
+    var oelt := TryGetParsed(cfg, data, 0);
     if oelt == None {
       return None;
     }
@@ -609,10 +412,11 @@ refines UniformSizedElementSeqMarshallingCommon(Element_Marshalling) {
     while i < len
       invariant i <= len
       invariant |lresult| == len as nat
-      invariant forall j: nat | j < i as nat :: ElementMarshalling.parsable(ElementData(data, j as uint64))
-      invariant forall j: nat | j < i as nat :: lresult[j] == ElementMarshalling.parse(ElementData(data, j as uint64))
+      invariant forall j: nat | j < i as nat :: gettable(cfg, data, j)
+      invariant forall j: nat | j < i as nat :: Elt.parsable(EltCfg(cfg), getData(cfg, data, j))
+      invariant forall j: nat | j < i as nat :: lresult[j] == getElt(cfg, data, j)
     {
-      oelt := ElementMarshalling.TryParse(ElementData(data, i));
+      oelt := TryGetParsed(cfg, data, i);
       if oelt == None {
         parsing_failed := true;
         break;
@@ -629,88 +433,360 @@ refines UniformSizedElementSeqMarshallingCommon(Element_Marshalling) {
       ovalue := Some(result);
     }
   }
+}
 
-  method Parsable(data: mseq<byte>) returns (p: bool)
+//////////////////////////////////////////////////////////////////////
+// Common parts of implementation of marshalling a sequence of items
+// that all have the same marshalled size.
+//
+// We omit the actual parsing and marshalling implementations so that
+// we can use the optimized integer packing code.
+//////////////////////////////////////////////////////////////////////
+
+abstract module UniformSizedElementSeqMarshalling(elementMarshalling: Marshalling)
+refines SeqMarshalling(elementMarshalling) {
+  import opened Mathematics
+  import Seq = Sequences
+  import opened Math
+  import NLarith
+
+  type Config = Elt.Config
+
+  predicate validConfig(cfg: Config) {
+    && Elt.validConfig(cfg)
+  }
+
+  function method EltCfg(cfg: Config) : Elt.Config {
+    cfg
+  }
+
+  function method UniformSize(cfg: Config) : uint64
+    requires validConfig(cfg)
+    ensures 0 < UniformSize(cfg)
+
+  predicate lengthable(cfg: Config, data: mseq<byte>)
   {
-    var len: uint64 := Length(data);
-    if len == 0 {
-      return true;
-    }
+    true
+  }
 
-    var i: uint64 := 0;
-    while i < len
-      invariant i <= len
-      invariant forall j: nat | j < i as nat :: ElementMarshalling.parsable(ElementData(data, j as uint64))
+  function slice_length(cfg: Config, slice: Slice) : nat
+    requires validConfig(cfg)
+    requires slice.WF()
+  {
+    NLarith.DivLe(|slice| as nat, UniformSize(cfg) as nat);
+    |slice| as nat / UniformSize(cfg) as nat
+  }
+
+  function length(cfg: Config, data: mseq<byte>) : nat
+    ensures slice_length(cfg, all(data))
+         == length(cfg, data)
+         <=  length(cfg, data) * UniformSize(cfg) as nat
+         <= |data| as nat
+  {
+    NLarith.DivLe(|data| as nat, UniformSize(cfg) as nat);
+    DivMulOrder(|data| as nat, UniformSize(cfg) as nat);
+    assert (|data| as nat / UniformSize(cfg) as nat) * 1 == |data| as nat / UniformSize(cfg) as nat;
+    if 1 < UniformSize(cfg) then
+      PosMulPreservesLe(1, UniformSize(cfg) as nat, |data| as nat / UniformSize(cfg) as nat);
+      |data| as nat / UniformSize(cfg) as nat
+    else
+      |data| as nat / UniformSize(cfg) as nat
+  }
+
+  method TryLength(cfg: Config, data: mseq<byte>) returns (olen: Option<uint64>)
+  {
+    NLarith.DivLe(|data| as nat, UniformSize(cfg) as nat);
+    olen := Some(|data| as uint64 / UniformSize(cfg));
+  }
+
+  method Lengthable(cfg: Config, data: mseq<byte>) returns (l: bool)
+  {
+    l := true;
+  }
+
+  method Length(cfg: Config, data: mseq<byte>) returns (len: uint64)
+    ensures len as nat == length(cfg, data)
+  {
+    NLarith.DivLe(|data| as nat, UniformSize(cfg) as nat);
+    len := |data| as uint64 / UniformSize(cfg);
+  }
+
+  lemma index_bounds_facts(cfg: Config, slice: Slice, idx: nat)
+    requires validConfig(cfg)
+    requires slice.WF()
+    requires idx < |slice| as nat / UniformSize(cfg) as nat
+    ensures 0 <=  idx * UniformSize(cfg) as nat
+              <  idx * UniformSize(cfg) as nat + UniformSize(cfg) as nat
+              == (idx + 1) * UniformSize(cfg) as nat
+              <=  |slice| as nat
+  {
+    NatMulNatIsNat(idx, UniformSize(cfg) as nat);
+    PosMulPreservesOrder(idx, idx + 1, UniformSize(cfg) as nat);
+    NLarith.DistributeLeft(idx, 1, UniformSize(cfg) as nat);
+    DivMulOrder(|slice| as nat, UniformSize(cfg) as nat);
+    if idx + 1 < slice_length(cfg, slice) as nat {
+      PosMulPreservesOrder(idx + 1, slice_length(cfg, slice), UniformSize(cfg) as nat);
+    }
+  }
+
+  predicate gettable(cfg: Config, data: mseq<byte>, idx: nat) {
+    idx < length(cfg, data)
+  }
+
+  function get(cfg: Config, slice: Slice, data: mseq<byte>, idx: nat) : (eslice: Slice)
+    ensures |eslice| == UniformSize(cfg)
+  {
+    index_bounds_facts(cfg, slice, idx as nat);
+    slice.sub(idx as uint64 * UniformSize(cfg), idx as uint64 * UniformSize(cfg) + UniformSize(cfg))
+  }
+
+  method TryGet(cfg: Config, slice: Slice, data: mseq<byte>, idx: uint64) returns (oeslice: Option<Slice>)
+  {
+    var len := Length(cfg, slice.I(data));
+    if idx < len {
+      index_bounds_facts(cfg, slice, idx as nat);
+      oeslice := Some(slice.sub(idx * UniformSize(cfg), idx * UniformSize(cfg) + UniformSize(cfg)));
+    } else {
+      oeslice := None;
+    }
+  }
+
+  method Gettable(cfg: Config, data: mseq<byte>, idx: uint64) returns (g: bool)
+  {
+    var len := Length(cfg, data);
+    g := idx < len;
+  }
+
+  method Get(cfg: Config, slice: Slice, data: mseq<byte>, idx: uint64) returns (eslice: Slice)
+  {
+    index_bounds_facts(cfg, slice, idx as nat);
+    eslice := slice.sub(idx * UniformSize(cfg), idx * UniformSize(cfg) + UniformSize(cfg));
+  }
+
+  predicate settable(cfg: Config, data: mseq<byte>, idx: nat, value: Element) {
+    && idx < length(cfg, data)
+    && Elt.marshallable(EltCfg(cfg), value)
+    && Elt.size(EltCfg(cfg), value) == UniformSize(cfg)
+  }
+
+  method Settable(cfg: Config, data: mseq<byte>, idx: uint64, value: Element) returns (s: bool)
+  {
+    var len := Length(cfg, data);
+    var sz := Elt.Size(EltCfg(cfg), value);
+    return idx < len && sz == UniformSize(cfg);
+  }
+
+  method Set(cfg: Config, slice: Slice, linear inout data: mseq<byte>, idx: uint64, value: Element)
+  {
+    index_bounds_facts(cfg, slice, idx as nat);
+
+    var newend := Elt.Marshall(EltCfg(cfg), value, inout data, slice.start + idx * UniformSize(cfg));
+
+    forall i: nat | i != idx as nat && gettable(cfg, slice.I(old_data), i)
+      ensures getData(cfg, slice.I(data), i) == getData(cfg, slice.I(old_data), i)
     {
-      var p' := ElementMarshalling.Parsable(ElementData(data, i));
-      if p' == false {
-        return false;
+      index_bounds_facts(cfg, slice, i);
+
+      Seq.lemma_seq_slice_slice(data,
+        slice.start as nat,
+        slice.end as nat,
+        i * UniformSize(cfg) as nat,
+        i * UniformSize(cfg) as nat + UniformSize(cfg) as nat);
+      Seq.lemma_seq_slice_slice(old_data,
+        slice.start as nat,
+        slice.end as nat,
+        i * UniformSize(cfg) as nat,
+        i * UniformSize(cfg) as nat + UniformSize(cfg) as nat);
+
+      if i < idx as nat {
+        NLarith.MulPreservesLe(i + 1, idx as nat, UniformSize(cfg) as nat);
+      } else {
+        NLarith.MulPreservesLe(idx as nat + 1, i, UniformSize(cfg) as nat);
       }
-      i := i + 1;
     }
-    return true;
+
+    Seq.lemma_seq_slice_slice(data,
+      slice.start as nat,
+      slice.end as nat,
+      idx as nat * UniformSize(cfg) as nat,
+      idx as nat * UniformSize(cfg) as nat + UniformSize(cfg) as nat);
   }
 
-  method Parse(data: mseq<byte>) returns (value: UnmarshalledType) {
-    var len: uint64 := Length(data);
-    if len == 0 {
-      var empty: UnmarshalledType := [];
-      return empty;
-    }
-
-    // We get the first element by itself so we can call
-    // seq_alloc_init below.
-    var elt := ElementMarshalling.Parse(ElementData(data, 0));
-    linear var lresult := seq_alloc_init(len, elt);
-
-    var i: uint64 := 1;
-    while i < len
-      invariant i <= len
-      invariant |lresult| == len as nat
-      invariant forall j: nat | j < i as nat :: lresult[j] == ElementMarshalling.parse(ElementData(data, j as uint64))
-    {
-      elt := ElementMarshalling.Parse(ElementData(data, i));
-      mut_seq_set(inout lresult, i, elt);
-      i := i + 1;
-    }
-
-    var result: UnmarshalledType := seq_unleash(lresult);
-    value := result;
+  predicate resizable(cfg: Config, data: mseq<byte>, newlen: nat) {
+    false
   }
 
-  method Marshall(value: UnmarshalledType, linear data: mseq<byte>, start: uint64)
-    returns (linear newdata: mseq<byte>, end: uint64)
+  method Resizable(cfg: Config, data: mseq<byte>, newlen: uint64) returns (r: bool)
   {
-    newdata := data;
+    return false;
+  }
+
+  method Resize(cfg: Config, slice: Slice, linear inout data: mseq<byte>, newlen: uint64)
+  {
+    // This function requires false and hence cannot be called.
+  }
+
+  predicate marshallable(cfg: Config, value: UnmarshalledType)
+  {
+    && (forall i | 0 <= i < |value| :: Elt.marshallable(EltCfg(cfg), value[i]))
+    && (forall i | 0 <= i < |value| :: Elt.size(EltCfg(cfg), value[i]) == UniformSize(cfg))
+    && |value| * UniformSize(cfg) as nat < Uint64UpperBound()
+  }
+
+  lemma marshallable_prefix(cfg: Config, value: UnmarshalledType, len: nat)
+    requires validConfig(cfg)
+    requires marshallable(cfg, value)
+    requires len <= |value|
+    ensures marshallable(cfg, value[..len])
+
+  function size(cfg: Config, value: UnmarshalledType) : uint64
+  {
+    NatMulNatIsNat(|value|, UniformSize(cfg) as nat);
+    |value| as uint64 * UniformSize(cfg)
+  }
+
+  method Size(cfg: Config, value: UnmarshalledType) returns (sz: uint64)
+  {
+    sz := NLarith.Uint64Mult(|value| as uint64, UniformSize(cfg));
+  }
+
+  lemma parsing_extend(cfg: Config, data: mseq<byte>, edata: mseq<byte>)
+    requires validConfig(cfg)
+    requires parsable(cfg, data)
+    requires |data| == length(cfg, data) * UniformSize(cfg) as nat
+    requires Elt.parsable(EltCfg(cfg), edata)
+    requires |edata| == UniformSize(cfg) as nat
+    requires |data + edata| < Uint64UpperBound()
+    ensures parsable(cfg, data + edata)
+    ensures parse(cfg, data + edata) == parse(cfg, data) + [ Elt.parse(EltCfg(cfg), edata) ]
+  {
+    var extension := data + edata;
+    lemma_div_ind(|data|, UniformSize(cfg) as nat);
+    forall idx | 0 <= idx < length(cfg, data)
+      ensures getData(cfg, extension, idx) == getData(cfg, data, idx);
+    {
+      index_bounds_facts(cfg, all(data), idx);
+      Seq.lemma_seq_slice_slice(extension, 0, |data|, idx * UniformSize(cfg) as nat, idx * UniformSize(cfg) as nat + UniformSize(cfg) as nat);
+    }
+    assert getData(cfg, extension, length(cfg, data)) == edata;
+    assert parse(cfg, extension)[..length(cfg, data)] == parse(cfg, data);
+  }
+
+  method Marshall(cfg: Config, value: UnmarshalledType, linear inout data: mseq<byte>, start: uint64)
+    returns (end: uint64)
+  {
     var i: uint64 := 0;
     end := start;
+
+    forall l | 0 <= l < |value|
+      ensures marshallable(cfg, value[..l])
+    {
+      NLarith.MulPreservesLe(l, |value|, UniformSize(cfg) as nat);
+    }
+
     while i < |value| as uint64
       invariant i <= |value| as uint64
-      invariant |newdata| == |data|
-      invariant end as nat == start as nat + size(value[..i]) <= |newdata|
-      invariant forall j | 0 <= j < start :: newdata[j] == data[j]
-      invariant forall j | end as nat <= j < |data| :: newdata[j] == data[j]
-      invariant parsable(newdata[start..end])
-      invariant parse(newdata[start..end]) == value[..i]
+      invariant |data| as nat == |old_data|
+      invariant end as nat == start as nat + size(cfg, value[..i]) as nat <= |data| as nat
+      invariant forall j | 0 <= j < start :: data[j] == old_data[j]
+      invariant forall j | end as nat <= j < |old_data| :: data[j] == old_data[j]
+      invariant parsable(cfg, data[start..end])
+      invariant parse(cfg, data[start..end]) == value[..i]
     {
       ghost var oldend := end;
-      ghost var olddata := newdata[start..end];
+      ghost var olddata := data[start..end];
       if i as nat + 1 < |value| {
-        PosMulPreservesOrder(i as nat + 1, |value|, UniformSize() as nat);
+        PosMulPreservesOrder(i as nat + 1, |value|, UniformSize(cfg) as nat);
       }
 
-      NLarith.DistributeLeft(i as nat, 1, UniformSize() as nat);
-      newdata, end := ElementMarshalling.Marshall(value[i], newdata, end);
+      NLarith.DistributeLeft(i as nat, 1, UniformSize(cfg) as nat);
+      end := Elt.Marshall(EltCfg(cfg), value[i], inout data, end);
       i := i + 1;
 
-      assert newdata[start..oldend] == olddata;
-      parsing_extend(newdata[start..oldend], newdata[oldend..end]);
-      assert newdata[start..end] == newdata[start..oldend] + newdata[oldend..end];
+      assert data[start..oldend] == olddata;
+      parsing_extend(cfg, data[start..oldend], data[oldend..end]);
+      assert data[start..end] == data[start..oldend] + data[oldend..end];
       assert value[..i] == value[..i-1] + [ value[i-1] ];
     }
     assert value == value[..|value|];
   }
 }
+
+/////////////////////////////////////////////////////////////////
+// Implementation for marshalling a sequence of packable integers
+//
+// We could just use the UniformSized marshalling code further below,
+// but that would marshall each integer one at a time, which would
+// (presumably) be slower.
+/////////////////////////////////////////////////////////////////
+
+module IntegerSeqMarshalling(Int: NativePackedInt)
+refines UniformSizedElementSeqMarshalling(IntegerMarshalling(Int)) {
+
+  function method UniformSize(cfg: Config) : uint64 {
+    Int.Size()
+  }
+  
+  lemma parse_is_unpack_Seq(cfg: Config, data: mseq<byte>)
+    requires validConfig(cfg)
+    requires parsable(cfg, data)
+    ensures parse(cfg, data) == Int.unpack_Seq(data[..length(cfg, data) * Int.Size() as nat], length(cfg, data))
+  {
+    var len := length(cfg, data);
+    var value := Int.unpack_Seq(data[..len * Int.Size() as nat], len);
+    forall i | 0 <= i < |value|
+      ensures value[i] == parse(cfg, data)[i]
+    {
+      index_bounds_facts(cfg, all(data), i);
+      if i + 1 < len {
+        PosMulPreservesOrder(i + 1, len, Int.Size() as nat);
+      }
+      Seq.lemma_seq_slice_slice(data, 0, Int.Size() as nat * len as nat, i * Int.Size() as nat, (i+1) * Int.Size() as nat);
+      Seq.lemma_seq_slice_slice(data, i * UniformSize(cfg) as nat, (i + 1) * UniformSize(cfg) as nat, 0, Int.Size() as nat);
+    }
+  }
+
+  method TryParse(cfg: Config, data: mseq<byte>) returns (ovalue: Option<UnmarshalledType>)
+  {
+    var len := Length(cfg, data);
+    var value: mseq<Int.Integer> := Int.Cast_Seq(data, 0, len);
+    ovalue := Some(value);
+    assert parsable(cfg, data);
+    parse_is_unpack_Seq(cfg, data);
+  }
+
+  method Parsable(cfg: Config, data: mseq<byte>) returns (p: bool)
+  {
+    return true;
+  }
+
+  method Parse(cfg: Config, data: mseq<byte>) returns (value: UnmarshalledType)
+  {
+    var length := Length(cfg, data);
+    value := Int.Cast_Seq(data, 0, length);
+    parse_is_unpack_Seq(cfg, data);
+  }
+
+  method Marshall(cfg: Config, value: UnmarshalledType, linear inout data: mseq<byte>, start: uint64)
+    returns (end: uint64)
+  {
+    Int.Pack_Seq_into_ByteSeq(value, inout data, start);
+    var sz := Size(cfg, value);
+    end := start + sz;
+
+    assert parsable(cfg, data[start..end]);
+    parse_is_unpack_Seq(cfg, data[start..end]);
+    MulDivCancel(|value|, Int.Size() as nat);
+    Seq.lemma_seq_slice_slice(data, start as nat, end as nat, 0, length(cfg, data[start..end]) * Int.Size() as nat);
+  }
+}
+
+module Uint32SeqMarshalling refines IntegerSeqMarshalling(NativePackedUint32) {
+}
+
+module Uint64SeqMarshalling refines IntegerSeqMarshalling(NativePackedUint64) {
+}
+
 
 ////////////////////////////////////////////////////////////////////
 // Marshalling of sequences of uniform-sized elements, with a length
@@ -722,10 +798,7 @@ ResizableUniformSizedElementSeqMarshalling(LengthInt: NativePackedInt,
                                            elementMarshalling: Marshalling)
 refines SeqMarshalling(elementMarshalling) {
   import LengthMarshalling = IntegerMarshalling(LengthInt)
-  import USESM = UniformSizedElementSeqMarshallingCommon(elementMarshalling)
   import opened Mathematics
-  import opened LinearSequence_s
-  import opened LinearSequence_i
   import Seq = Sequences
   import NLarith
 
@@ -733,667 +806,662 @@ refines SeqMarshalling(elementMarshalling) {
     LengthInt.Size()
   }
 
-  function maxLength(data: mseq<byte>) : nat
-    requires sizeOfLengthField() as nat <= |data|
-  {
-    USESM.length(data[sizeOfLengthField()..])
-  }
-  
-  predicate lengthable'(data: mseq<byte>) {
-    && sizeOfLengthField() as nat <= |data|
-    && var ilen := LengthMarshalling.parse(data[..sizeOfLengthField()]);
-    && LengthInt.fitsInUint64(ilen)
-    && var len := LengthInt.toInt(ilen);
-    && len <= maxLength(data)
+  datatype Config = Config(totalSize: uint64, lengthCfg: LengthMarshalling.Config, eltCfg: Elt.Config)
+
+  predicate validConfig(cfg: Config) {
+    && sizeOfLengthField() <= cfg.totalSize
+    && LengthMarshalling.validConfig(cfg.lengthCfg)
+    && Elt.validConfig(cfg.eltCfg)
   }
 
-  function length(data: mseq<byte>) : nat
-    requires lengthable'(data)
-    ensures length(data) <=  length(data) * USESM.UniformSize() as nat <= |data| - sizeOfLengthField() as nat
+  function method EltCfg(cfg: Config) : Elt.Config {
+    cfg.eltCfg
+  }
+
+  function method UniformSize(cfg: Config) : uint64
+    requires validConfig(cfg)
+    ensures 0 < UniformSize(cfg)
+
+  function method maxLength(cfg: Config) : uint64
+    requires validConfig(cfg)
   {
-    var len := LengthInt.toInt(LengthMarshalling.parse(data[..sizeOfLengthField()]));
-    PosMulPreservesLe(len, (|data| - sizeOfLengthField() as nat) / USESM.UniformSize() as nat, USESM.UniformSize() as nat);
-    PosMulPreservesLe(1, USESM.UniformSize() as nat, len);
+    NLarith.DivLe(cfg.totalSize as nat - sizeOfLengthField() as nat, UniformSize(cfg) as nat);
+    (cfg.totalSize - sizeOfLengthField()) / UniformSize(cfg)
+  }
+
+  predicate lengthable(cfg: Config, data: mseq<byte>) {
+    && cfg.totalSize as nat <= |data|
+    && var ilen := LengthMarshalling.parse(cfg.lengthCfg, data[..sizeOfLengthField()]);
+    && LengthInt.fitsInUint64(ilen)
+  }
+
+  function length(cfg: Config, data: mseq<byte>) : nat
+  {
+    var len := LengthInt.toInt(LengthMarshalling.parse(cfg.lengthCfg, data[..sizeOfLengthField()]));
+    NLarith.DivLe(|data| - sizeOfLengthField() as nat,  UniformSize(cfg) as nat);
     len
   }
 
-  predicate lengthable(data: mseq<byte>) {
-    lengthable'(data)
-  }
-
-  lemma index_bounds_facts(data: mseq<byte>, idx: nat)
-    requires sizeOfLengthField() as nat <= |data|
-    requires idx < maxLength(data)
+  lemma index_bounds_facts(cfg: Config, idx: nat)
+    requires validConfig(cfg)
+    requires idx < maxLength(cfg) as nat
     ensures
-    0 <=  sizeOfLengthField() as nat + idx * USESM.UniformSize() as nat
-      <  sizeOfLengthField() as nat + idx * USESM.UniformSize() as nat + USESM.UniformSize() as nat
-      == sizeOfLengthField() as nat + (idx + 1) * USESM.UniformSize() as nat
-      <=  sizeOfLengthField() as nat + maxLength(data) * USESM.UniformSize() as nat
-      <=  |data|
+         sizeOfLengthField() as nat
+      <=  sizeOfLengthField() as nat + idx * UniformSize(cfg) as nat
+      <  sizeOfLengthField() as nat + idx * UniformSize(cfg) as nat + UniformSize(cfg) as nat
+      == sizeOfLengthField() as nat + (idx + 1) * UniformSize(cfg) as nat
+      <=  sizeOfLengthField() as nat + maxLength(cfg) as nat * UniformSize(cfg) as nat
+      <=  cfg.totalSize as nat
   {
-    NatMulNatIsNat(idx, USESM.UniformSize() as nat);
-    NLarith.DistributeLeft(idx, 1, USESM.UniformSize() as nat);
-    if idx + 1 < maxLength(data) {
-      PosMulPreservesOrder(idx + 1, maxLength(data), USESM.UniformSize() as nat);
+    NatMulNatIsNat(idx, UniformSize(cfg) as nat);
+    NLarith.DistributeLeft(idx, 1, UniformSize(cfg) as nat);
+    DivMulOrder(cfg.totalSize as nat - sizeOfLengthField() as nat, UniformSize(cfg) as nat);
+    if idx + 1 < maxLength(cfg) as nat {
+      PosMulPreservesOrder(idx + 1, maxLength(cfg) as nat, UniformSize(cfg) as nat);
     }
   }
 
-  method TryLength(data: mseq<byte>) returns (olen: Option<uint64>)
-    ensures olen.Some? ==> olen.value as nat == length(data)
+  method TryLength(cfg: Config, data: mseq<byte>) returns (olen: Option<uint64>)
   {
-    if LengthInt.Size() <= |data| as uint64 {
-      var l' := LengthMarshalling.Parse(data[..sizeOfLengthField()]);
-      if LengthInt.fitsInUint64(l') {
-        var l: uint64 := LengthInt.toUint64(l');
-        var maxl := USESM.Length(data[sizeOfLengthField()..]);
-        if l <= maxl {
-          if l < maxl {
-            index_bounds_facts(data, l as nat);
-          }
-          MulDivCancel(l as nat, USESM.UniformSize() as nat);
-          NatMulNatIsNat(l as nat, USESM.UniformSize() as nat);
-          olen := Some(l);
-        } else {
-          olen := None;
-        }
-      } else {
-        olen := None;
-      }
+    if |data| as uint64 < cfg.totalSize {
+      return None;
+    }
+    var l' := LengthMarshalling.Parse(cfg.lengthCfg, data[..sizeOfLengthField()]);
+    if LengthInt.fitsInUint64(l') {
+      return Some(LengthInt.toUint64(l'));
     } else {
       olen := None;
     }
   }
 
-  method Lengthable(data: mseq<byte>) returns (l: bool) {
-    var olen := TryLength(data);
+  method Lengthable(cfg:Config, data: mseq<byte>) returns (l: bool) {
+    var olen := TryLength(cfg, data);
     return olen.Some?;
+  }
+
+  method Length(cfg: Config, data: mseq<byte>) returns (len: uint64)
+  {
+    var l := LengthMarshalling.Parse(cfg.lengthCfg, data[..sizeOfLengthField()]);
+    len := LengthInt.toUint64(l);
+    ghost var ghosty := true;
+    if ghosty && len as nat < maxLength(cfg) as nat {
+      index_bounds_facts(cfg, len as nat);
+    }
+    MulDivCancel(len as nat, UniformSize(cfg) as nat);
+    NatMulNatIsNat(len as nat, UniformSize(cfg) as nat);
+  }
+
+  predicate gettable(cfg: Config, data: mseq<byte>, idx: nat) {
+    && lengthable(cfg, data)
+    && idx < maxLength(cfg) as nat
+  }
+
+  function get(cfg: Config, slice: Slice, data: mseq<byte>, idx: nat) : (eslice: Slice)
+  {
+    index_bounds_facts(cfg, idx as nat);
+    slice.sub(sizeOfLengthField() + idx as uint64 * UniformSize(cfg),
+      sizeOfLengthField() + idx as uint64 * UniformSize(cfg) + UniformSize(cfg))
+  }
+
+  method TryGet(cfg: Config, slice: Slice, data: mseq<byte>, idx: uint64) returns (oeslice: Option<Slice>) {
+    var olen := TryLength(cfg, slice.I(data));
+    if olen == None {
+      return None;
+    }
+    var mlen := maxLength(cfg);
+    if idx < mlen {
+      index_bounds_facts(cfg, idx as nat);
+      NatMulNatIsNat(idx as nat, UniformSize(cfg) as nat);
+      oeslice := Some(slice.sub(sizeOfLengthField() + idx * UniformSize(cfg), sizeOfLengthField() + idx * UniformSize(cfg) + UniformSize(cfg)));
+    } else {
+      oeslice := None;
+    }
+  }
+
+  method Gettable(cfg: Config, data: mseq<byte>, idx: uint64) returns (g: bool) {
+    var olen := TryLength(cfg, data);
+    return olen != None && idx < maxLength(cfg);
+  }
+
+  method Get(cfg: Config, slice: Slice, data: mseq<byte>, idx: uint64) returns (eslice: Slice) {
+    index_bounds_facts(cfg, idx as nat);
+    NatMulNatIsNat(idx as nat, UniformSize(cfg) as nat);
+    return slice.sub(sizeOfLengthField() + idx * UniformSize(cfg), sizeOfLengthField() + idx * UniformSize(cfg) + UniformSize(cfg));
+  }
+
+  predicate settable(cfg: Config, data: mseq<byte>, idx: nat, value: Element) {
+    && lengthable(cfg, data)
+    && idx < maxLength(cfg) as nat
+    && Elt.size(EltCfg(cfg), value) == UniformSize(cfg)
+  }
+
+  method Settable(cfg: Config, data: mseq<byte>, idx: uint64, value: Element) returns (s: bool)
+  {
+    var olen := TryLength(cfg, data);
+    var sz := Elt.Size(EltCfg(cfg), value);
+    return
+      && olen != None
+      && idx < maxLength(cfg)
+      && sz == UniformSize(cfg);
+  }
+
+  method Set(cfg: Config, slice: Slice, linear inout data: mseq<byte>, idx: uint64, value: Element)
+  {
+    var newend;
+    index_bounds_facts(cfg, idx as nat);
+    NatMulNatIsNat(idx as nat, UniformSize(cfg) as nat);
+    newend := Elt.Marshall(EltCfg(cfg), value, inout data, slice.start + sizeOfLengthField() + idx * UniformSize(cfg));
+
+    assert slice.I(data)[..sizeOfLengthField()] == slice.I(old_data)[..sizeOfLengthField()];
+
+    forall i: nat | i != idx as nat && gettable(cfg, slice.I(old_data), i)
+      ensures getData(cfg, slice.I(data), i) == getData(cfg, slice.I(old_data), i)
+    {
+      index_bounds_facts(cfg, i);
+      Seq.lemma_seq_slice_slice(data,
+        slice.start as nat,
+        slice.end as nat,
+        sizeOfLengthField() as nat + i * UniformSize(cfg) as nat,
+        sizeOfLengthField() as nat + i * UniformSize(cfg) as nat + UniformSize(cfg) as nat);
+      Seq.lemma_seq_slice_slice(old_data,
+        slice.start as nat,
+        slice.end as nat,
+        sizeOfLengthField() as nat + i * UniformSize(cfg) as nat,
+        sizeOfLengthField() as nat + i * UniformSize(cfg) as nat + UniformSize(cfg) as nat);
+
+      if i < idx as nat {
+        NLarith.MulPreservesLe(i + 1, idx as nat, UniformSize(cfg) as nat);
+        calc {
+          getData(cfg, slice.I(data), i);
+          data[slice.start..slice.end]
+            [sizeOfLengthField() as nat + i * UniformSize(cfg) as nat..
+             sizeOfLengthField() as nat + i * UniformSize(cfg) as nat + UniformSize(cfg) as nat];
+
+          old_data[slice.start..slice.end]
+            [sizeOfLengthField() as nat + i * UniformSize(cfg) as nat..
+             sizeOfLengthField() as nat + i * UniformSize(cfg) as nat + UniformSize(cfg) as nat];
+          getData(cfg, slice.I(old_data), i);
+        }
+      } else {
+        NLarith.MulPreservesLe(idx as nat + 1, i, UniformSize(cfg) as nat);
+      }
+    }
+
+    Seq.lemma_seq_slice_slice(data,
+      slice.start as nat,
+      slice.end as nat,
+      sizeOfLengthField() as nat + idx as nat * UniformSize(cfg) as nat,
+      sizeOfLengthField() as nat + idx as nat * UniformSize(cfg) as nat + UniformSize(cfg) as nat);
+  }
+
+  predicate resizable(cfg: Config, data: mseq<byte>, newlen: nat) {
+    && lengthable(cfg, data)
+    && newlen <= maxLength(cfg) as nat
+    && LengthInt.fitsInInteger(newlen as uint64)
+  }
+
+  method Resizable(cfg: Config, data: mseq<byte>, newlen: uint64) returns (r: bool)
+  {
+    var l := Lengthable(cfg, data);
+    return
+      && l
+      && newlen <= maxLength(cfg)
+      && LengthInt.fitsInInteger(newlen);
+  }
+
+  method Resize(cfg: Config, slice: Slice, linear inout data: mseq<byte>, newlen: uint64)
+  {
+    var newend := LengthMarshalling.Marshall(cfg.lengthCfg, LengthInt.fromUint64(newlen), inout data, slice.start);
+
+    assert data[slice.start..slice.end][..LengthInt.Size()] == data[slice.start..slice.start + LengthInt.Size()];
+    LengthInt.fromtoInverses();
+
+    forall i: nat | gettable(cfg, slice.I(old_data), i)
+      ensures getData(cfg, slice.I(data), i) == getData(cfg, slice.I(old_data), i)
+    {
+      index_bounds_facts(cfg, i);
+      Seq.lemma_seq_slice_slice(data,
+        slice.start as nat,
+        slice.end as nat,
+        sizeOfLengthField() as nat + i * UniformSize(cfg) as nat,
+        sizeOfLengthField() as nat + i * UniformSize(cfg) as nat + UniformSize(cfg) as nat);
+      Seq.lemma_seq_slice_slice(old_data,
+        slice.start as nat,
+        slice.end as nat,
+        sizeOfLengthField() as nat + i * UniformSize(cfg) as nat,
+        sizeOfLengthField() as nat + i * UniformSize(cfg) as nat + UniformSize(cfg) as nat);
+
+        calc {
+          getData(cfg, slice.I(data), i);
+          data[slice.start..slice.end]
+            [sizeOfLengthField() as nat + i * UniformSize(cfg) as nat..
+            sizeOfLengthField() as nat + i * UniformSize(cfg) as nat + UniformSize(cfg) as nat];
+
+          old_data[slice.start..slice.end]
+            [sizeOfLengthField() as nat + i * UniformSize(cfg) as nat..
+            sizeOfLengthField() as nat + i * UniformSize(cfg) as nat + UniformSize(cfg) as nat];
+            getData(cfg, slice.I(old_data), i);
+        }
+    }
+  }
+
+  predicate marshallable(cfg: Config, value: UnmarshalledType) {
+    && (forall i | 0 <= i < |value| :: Elt.marshallable(EltCfg(cfg), value[i]))
+    && (forall i | 0 <= i < |value| :: Elt.size(EltCfg(cfg), value[i]) == UniformSize(cfg))
+    && LengthInt.fitsInInteger(|value| as uint64)
+    && sizeOfLengthField() as nat + |value| * UniformSize(cfg) as nat <= cfg.totalSize as nat
+  }
+
+  function size(cfg: Config, value: UnmarshalledType) : uint64 {
+    cfg.totalSize
+  }
+
+  method Size(cfg: Config, value: UnmarshalledType) returns (sz: uint64) {
+    return cfg.totalSize;
+  }
+
+  method Marshall(cfg: Config, value: UnmarshalledType, linear inout data: mseq<byte>, start: uint64)
+    returns (end: uint64)
+  {
+    end := start + cfg.totalSize;
+    var slice := Slice(start, end);
+    var ilen := LengthInt.fromUint64(|value| as uint64);
+    var dummy := LengthMarshalling.Marshall(cfg.lengthCfg, ilen, inout data, start);
+
+    LengthInt.fromtoInverses();
+    Seq.lemma_seq_slice_slice(data,
+      start as nat,
+      end as nat,
+      0,
+      sizeOfLengthField() as nat);
+    assert lengthable(cfg, data[start..end]);
+    assert length(cfg, data[start..end]) == |value|;
+
+    InequalityMoveDivisor(|value|, cfg.totalSize as nat - sizeOfLengthField() as nat, UniformSize(cfg) as nat);
+
+    var i: uint64 := 0;
+    while i < |value| as uint64
+      invariant i <= |value| as uint64
+      invariant |data| == |old_data|
+      invariant forall j | 0 <= j < start :: data[j] == old_data[j]
+      invariant forall j | end as nat <= j < |old_data| :: data[j] == old_data[j]
+      invariant lengthable(cfg, data[start..end])
+      invariant length(cfg, data[start..end]) == |value|
+      invariant forall j | 0 <= j < i :: gettable(cfg, data[start..end], j as nat)
+      invariant forall j | 0 <= j < i :: Elt.parsable(EltCfg(cfg), getData(cfg, data[start..end], j as nat))
+      invariant forall j | 0 <= j < i :: getElt(cfg, data[start..end], j as nat) == value[j]
+      invariant forall j | 0 <= j < |value| :: settable(cfg, data[start..end], j, value[j])
+    {
+      ghost var olddata := data;
+      Set(cfg, slice, inout data, i, value[i]);
+      i := i + 1;
+      assert forall j | 0 <= j < i - 1 :: preservesEntry(cfg, olddata[start..end], j as nat, data[start..end]);
+    }
+    assert value == value[..|value|];
+
+  }
+}
+
+
+// Implementation for marshalling a sequence of packable integers
+
+// We could just use the UniformSized marshalling code further below,
+// but that would marshall each integer one at a time, which would
+// (presumably) be slower.
+
+
+module ResizableIntegerSeqMarshalling(lengthInt: NativePackedInt, Int: NativePackedInt)
+refines ResizableUniformSizedElementSeqMarshalling(lengthInt, IntegerMarshalling(Int)) {
+
+  function method UniformSize(cfg: Config) : uint64 {
+    Int.Size()
+  }
+
+  lemma parse_is_unpack_Seq(cfg: Config, data: mseq<byte>)
+    requires validConfig(cfg)
+    requires parsable(cfg, data)
+    ensures parse(cfg, data) == Int.unpack_Seq(data[sizeOfLengthField()..sizeOfLengthField() as nat + length(cfg, data) * Int.Size() as nat], length(cfg, data))
+  {
+    var len := length(cfg, data);
+    var value := Int.unpack_Seq(data[sizeOfLengthField()..sizeOfLengthField() as nat + len * Int.Size() as nat], len);
+    forall i | 0 <= i < |value|
+      ensures value[i] == parse(cfg, data)[i]
+    {
+      index_bounds_facts(cfg, i);
+      if i + 1 < len {
+        PosMulPreservesOrder(i + 1, len, Int.Size() as nat);
+      }
+      Seq.lemma_seq_slice_slice(data, 0, Int.Size() as nat * len as nat, i * Int.Size() as nat, (i+1) * Int.Size() as nat);
+      Seq.lemma_seq_slice_slice(data, i * UniformSize(cfg) as nat, (i + 1) * UniformSize(cfg) as nat, 0, Int.Size() as nat);
+    }
+  }
+
+  method TryParse(cfg: Config, data: mseq<byte>) returns (ovalue: Option<UnmarshalledType>)
+  {
+    var len := Length(cfg, data);
+    var value: mseq<Int.Integer> := Int.Cast_Seq(data, 0, len);
+    ovalue := Some(value);
+    assert parsable(cfg, data);
+    parse_is_unpack_Seq(cfg, data);
+  }
+
+  method Parsable(cfg: Config, data: mseq<byte>) returns (p: bool)
+  {
+    return true;
+  }
+
+  method Parse(cfg: Config, data: mseq<byte>) returns (value: UnmarshalledType)
+  {
+    var length := Length(cfg, data);
+    value := Int.Cast_Seq(data, 0, length);
+    parse_is_unpack_Seq(cfg, data);
+  }
+
+  method Marshall(cfg: Config, value: UnmarshalledType, linear inout data: mseq<byte>, start: uint64)
+    returns (end: uint64)
+  {
+    Int.Pack_Seq_into_ByteSeq(value, inout data, start);
+    var sz := Size(cfg, value);
+    end := start + sz;
+
+    assert parsable(cfg, data[start..end]);
+    parse_is_unpack_Seq(cfg, data[start..end]);
+    MulDivCancel(|value|, Int.Size() as nat);
+    Seq.lemma_seq_slice_slice(data, start as nat, end as nat, 0, length(cfg, data[start..end]) * Int.Size() as nat);
+  }
+}
+
+// module ResizableUint32SeqMarshalling refines ResizableIntegerSeqMarshalling(NativePackedUint64, NativePackedUint32) {
+// }
+
+// module ResizableUint64SeqMarshalling refines ResizableIntegerSeqMarshalling(NativePackedUint64, NativePackedUint64) {
+// }
+
+
+//////////////////////////////////////////////////////////////////////
+// Implementation of marshalling a general sequence of items
+//////////////////////////////////////////////////////////////////////
+
+module VariableSizedElementSeqMarshalling(LengthInt: NativePackedInt, BoundaryInt: NativePackedInt, eMarshalling: Marshalling)
+refines SeqMarshalling(eMarshalling) {
+  import BoundarySeqMarshalling = ResizableUniformSizedElementSeqMarshalling(LengthInt, IntegerMarshalling(BoundaryInt))
+  import opened Sequences
+  import opened Mathematics
+  import NLarith
+
+  type LengthType = LengthInt.Integer
+  type Boundary = BoundaryInt.Integer
+  type BoundaryTable = mseq<Boundary>
+
+  // INTERNAL FUNCTIONS
+
+  function method sizeOfLengthField() : uint64 {
+    BoundarySeqMarshalling.sizeOfLengthField()
+  }
+
+  function method sizeOfBoundaryEntry() : uint64 {
+    BoundaryInt.Size()
+  }
+
+  function maxLength(data: mseq<byte>) : nat
+    ensures maxLength(data) <= |data|
+  {
+    BoundarySeqMarshalling.maxLength(data)
+  }
+
+  predicate lengthable(data: mseq<byte>)
+  {
+    BoundarySeqMarshalling.lengthable(data)
+  }
+
+  function length(data: mseq<byte>) : nat
+    requires lengthable(data)
+  {
+    BoundarySeqMarshalling.length(data)
+  }
+
+  function sizeOfTable(len: nat) : nat {
+    NatMulNatIsNat(len, sizeOfBoundaryEntry() as nat);
+    sizeOfLengthField() as nat + len * sizeOfBoundaryEntry() as nat
+  }
+
+  predicate tableable(data: mseq<byte>)
+    ensures tableable(data) ==> lengthable(data)
+    ensures tableable(data) ==> length(data) <= |data|
+  {
+    BoundarySeqMarshalling.parsable(data)
+  }
+
+  function btable(data: mseq<byte>) : mseq<BoundaryInt.Integer>
+    requires tableable(data)
+    ensures |btable(data)| == length(data)
+  {
+    BoundarySeqMarshalling.parse(data)
+  }
+
+  function table(data: mseq<byte>) : mseq<int>
+    requires tableable(data)
+  {
+    var bt := btable(data);
+    seq(|bt|, i requires 0 <= i < |bt| => BoundaryInt.toInt(bt[i]))
+  }
+
+  function ElementDataBegin(data: mseq<byte>, i: nat) : int
+    requires tableable(data)
+    requires i < length(data)
+  {
+    var t := table(data);
+    t[i]
+  }
+
+  function ElementDataEnd(data: mseq<byte>, i: nat) : int
+    requires tableable(data)
+    requires i < length(data)
+  {
+    var t := table(data);
+    if i == 0 then
+      |data|
+    else
+      t[i-1]
+  }
+
+  predicate validTableEntry(data: mseq<byte>, i: nat)
+    requires tableable(data)
+    requires i < length(data)
+  {
+    sizeOfTable(length(data)) <= ElementDataBegin(data, i) <= ElementDataEnd(data, i) <= |data|
+  }
+
+  predicate validTable(data: mseq<byte>)
+    requires tableable(data)
+  {
+    forall i | 0 <= i < length(data) :: validTableEntry(data, i)
+  }
+
+  function ElementData(data: mseq<byte>, i: nat) : mseq<byte>
+    requires tableable(data)
+    requires i < length(data)
+    requires validTableEntry(data, i)
+  {
+    data[ElementDataBegin(data, i) .. ElementDataEnd(data, i)]
+  }
+
+  predicate parsable(data: mseq<byte>)
+  {
+    && tableable(data)
+    && validTable(data)
+    && forall i | 0 <= i < length(data) :: ElementMarshalling.parsable(ElementData(data, i))
+  }
+
+  function parse(data: mseq<byte>) : UnmarshalledType
+  {
+    seq(length(data), i requires 0 <= i < length(data) => ElementMarshalling.parse(ElementData(data, i)))
+  }
+
+  method TryLength(data: mseq<byte>) returns (olen: Option<uint64>)
+    ensures olen.Some? ==> olen.value as nat == length(data)
+  {
+    olen := BoundarySeqMarshalling.TryLength(data);
+  }
+
+  method TryTable(data: mseq<byte>) returns (otable: Option<mseq<BoundaryInt.Integer>>)
+    ensures tableable(data) <==> otable.Some?
+    ensures tableable(data) ==> otable.value == btable(data)
+  {
+    var olen := TryLength(data);
+    if olen == None {
+      return None;
+    }
+    var len := olen.value;
+    var td := data[sizeOfLengthField()..sizeOfLengthField() + len * sizeOfBoundaryEntry()];
+    var t := BoundarySeqMarshalling.Parse(td);
+    otable := Some(t);
+  }
+
+  method TryParse(data: mseq<byte>) returns (ovalue: Option<UnmarshalledType>)
+  {
+    var otable := TryTable(data);
+    if otable == None {
+      return None;
+    }
+    var table := otable.value;
+    var len := |table| as uint64;
+    if len == 0 {
+      var empty: UnmarshalledType := [];
+      return Some(empty);
+    }
+    if !BoundaryInt.fitsInUint64(table[0]) || BoundaryInt.toUint64(table[0]) < sizeOfLengthField() + len * sizeOfBoundaryEntry() || |data| as uint64 < BoundaryInt.toUint64(table[0]) {
+      assert !validTable(data);
+      return None;
+    }
+
+    // We get the first element by itself so we can call
+    // seq_alloc_init below.
+    var oelt := ElementMarshalling.TryParse(data[BoundaryInt.toUint64(table[0])..]);
+    if oelt == None {
+      assert !ElementMarshalling.parsable(ElementData(data, 0));
+      return None;
+    }
+    linear var lresult := seq_alloc_init(len, oelt.value);
+
+    var i: uint64 := 1;
+    var parsing_failed := false;
+    while i < len
+      invariant i <= len
+      invariant |lresult| == len as nat
+      invariant forall j: nat | j < i as nat :: validTableEntry(data, j)
+      invariant forall j: nat | j < i as nat :: ElementMarshalling.parsable(ElementData(data, j))
+      invariant forall j: nat | j < i as nat :: lresult[j] == ElementMarshalling.parse(ElementData(data, j))
+    {
+      var ti := BoundaryInt.toUint64(table[i]);
+      var tim1 := BoundaryInt.toUint64(table[i-1]);
+      if ti < sizeOfLengthField() + len * sizeOfBoundaryEntry() || |data| as uint64 < ti || tim1 < ti {
+        parsing_failed := true;
+        break;
+      }
+      oelt := ElementMarshalling.TryParse(data[ti..tim1]);
+      if oelt == None {
+        parsing_failed := true;
+        break;
+      }
+      mut_seq_set(inout lresult, i, oelt.value);
+      i := i + 1;
+    }
+
+    var result: UnmarshalledType := seq_unleash(lresult);
+
+    if parsing_failed {
+      ovalue := None;
+    } else {
+      ovalue := Some(result);
+    }
+
+  }
+
+  function get(data: mseq<byte>, idx: nat) : mseq<byte>
+    requires gettable(data, idx)
+  {
+    structGet(partialParse(data), idx)
+  }
+
+  method TryGet(data: mseq<byte>, idx: uint64) returns (oedata: Option<mseq<byte>>)
+  {
+    var ostruct := PartialParse(data);
+    if ostruct == None || |ostruct.value.boundaries| as uint64 <= idx {
+      return None;
+    }
+    var struct := ostruct.value;
+
+    var start := BoundarySeqMarshalling.Int.toUint64(struct.boundaries[idx]);
+    var end := |struct.elements| as uint64;
+    if 0 < idx {
+      end := BoundarySeqMarshalling.Int.toUint64(struct.boundaries[idx]);
+    }
+
+    if start <= end <= |struct.elements| as uint64 {
+      oedata := Some(struct.elements[start..end]);
+    } else {
+      oedata := None;
+    }
+
+  }
+
+  method Gettable(data: mseq<byte>, idx: uint64) returns (g: bool)
+  {
+    var oedata := TryGet(data, idx);
+    return oedata.Some?;
+  }
+
+  method Get(data: mseq<byte>, idx: uint64) returns (edata: mseq<byte>)
+  {
+    var oedata := TryGet(data, idx);
+    return oedata.value;
+  }
+
+  method PartialParse(data: mseq<byte>) returns (oresult : Option<Structure>)
+    ensures oresult.Some? <==> tableable(data)
+    ensures tableable(data) ==> oresult.value == partialParse(data)
+  {
+    var olen := TryLength(data);
+    if olen == None {
+      return None;
+    }
+    var len := olen.value;
+
+    var tbdata := data[LengthMarshalling.Int.Size()..LengthMarshalling.Int.Size() + len * BoundarySeqMarshalling.Int.Size()];
+    var table := BoundarySeqMarshalling.Parse(tbdata);
+    var esdata := data[LengthMarshalling.Int.Size()..];
+    oresult := Some(Structure(table, esdata));
+  }
+
+
+  method TryLength(data: mseq<byte>) returns (olen: Option<uint64>)
+  {
+    if LengthMarshalling.Int.Size() <= |data| as uint64 {
+      var l := LengthMarshalling.Parse(data[..LengthMarshalling.Int.Size()]);
+      olen := Some(LengthMarshalling.Int.toUint64(l));
+    } else {
+      olen := None;
+    }
+  }
+
+  method Lengthable(data: mseq<byte>) returns (l: bool)
+  {
+    l := LengthMarshalling.Int.Size() <= |data| as uint64;
   }
 
   method Length(data: mseq<byte>) returns (len: uint64)
     ensures len as nat == length(data)
   {
-    var l := LengthMarshalling.Parse(data[..sizeOfLengthField()]);
-    len := LengthInt.toUint64(l);
-    if len as nat < maxLength(data) {
-      index_bounds_facts(data, len as nat);
-    }
-    MulDivCancel(len as nat, USESM.UniformSize() as nat);
-    NatMulNatIsNat(len as nat, USESM.UniformSize() as nat);
+    var l := LengthMarshalling.Parse(data[..LengthMarshalling.Int.Size()]);
+    len := LengthMarshalling.Int.toUint64(l);
   }
 
-  function method ElementData(data: mseq<byte>, idx: uint64) : mseq<byte>
-    requires sizeOfLengthField() as nat <= |data|
-    requires idx as nat < maxLength(data)
+
+  predicate gettable(data: mseq<byte>, idx: nat)
   {
-    USESM.ElementData(data[sizeOfLengthField()..], idx)
-  }
-
-  predicate gettable(data: mseq<byte>, idx: nat) {
-    && lengthable(data)
-    && var len := length(data);
-    && USESM.gettable(data[sizeOfLengthField() as nat..sizeOfLengthField() as nat + len * USESM.UniformSize() as nat], idx)
-  }
-
-  method TryGet(data: mseq<byte>, idx: uint64) returns (oedata: Option<mseq<byte>>) {
-    var olen := TryLength(data);
-    if olen == None {
-      return None;
-    }
-    var len := olen.value;
-    assert sizeOfLengthField() as nat + (len as nat) * (USESM.UniformSize() as nat) < Uint64UpperBound();
-    oedata := USESM.TryGet(data[sizeOfLengthField()..sizeOfLengthField() + len * USESM.UniformSize()], idx);
-    if parsable(data) {
-      parse_length(data);
-    }
-  }
-
-  method Gettable(data: mseq<byte>, idx: uint64) returns (g: bool) {
-    var olen := TryLength(data);
-    if olen == None {
-      return false;
-    }
-    var len := olen.value;
-    g := USESM.Gettable(data[sizeOfLengthField()..sizeOfLengthField() + len * USESM.UniformSize()], idx);
-  }
-
-  method Get(data: mseq<byte>, idx: uint64) returns (edata: mseq<byte>) {
-    var len := Length(data);
-    edata := USESM.Get(data[sizeOfLengthField()..sizeOfLengthField() + len * USESM.UniformSize()], idx);
-  }
-
-  predicate settable(data: mseq<byte>, idx: nat, value: Element) {
-    && lengthable(data)
-    && idx < length(data)
-    && ElementMarshalling.marshallable(value)
-    && ElementMarshalling.size(value) == USESM.UniformSize() as nat
-  }
-
-  method Settable(data: mseq<byte>, idx: uint64, value: Element) returns (s: bool)
-    requires ElementMarshalling.marshallable(value)
-    requires ElementMarshalling.size(value) < Uint64UpperBound()
-    ensures s == settable(data, idx as nat, value)
-  {
-    var olen := TryLength(data);
-    if olen == None {
-      return false;
-    }
-    var len := olen.value;
-    var sz := ElementMarshalling.Size(value);
-    return idx < len && sz == USESM.UniformSize();
-  }
-
-  method Set(linear data: mseq<byte>, start: uint64, end: uint64, idx: uint64, value: Element)
-    returns (linear newdata: mseq<byte>)
-    requires start as nat <= end as nat <= |data|
-    requires settable(data[start..end], idx as nat, value)
-    ensures |newdata| == |data|
-    ensures forall i | 0 <= i < start :: newdata[i] == data[i]
-    ensures forall i | end as nat <= i < |newdata| :: newdata[i] == data[i]
-    ensures lengthable(newdata[start..end])
-    ensures length(newdata[start..end]) == length(data[start..end])
-    ensures parsable(data[start..end]) ==> parsable(newdata[start..end])
-    ensures parsable(data[start..end]) ==> |parse(newdata[start..end])| == |parse(data[start..end])|
-    ensures parsable(data[start..end]) ==> idx as nat < |parse(data[start..end])|
-    ensures parsable(data[start..end]) ==> parse(newdata[start..end]) == parse(data[start..end])[idx as nat := value]
-  {
-    var substart := start + sizeOfLengthField();
-    USESM.index_bounds_facts(data[substart..end], idx as nat);
-
-    var newend;
-    newdata, newend := ElementMarshalling.Marshall(value, data, substart + idx * USESM.UniformSize());
-
-    assert newdata[start..end][..sizeOfLengthField()] == data[start..end][..sizeOfLengthField()];
-
-    if parsable(data[start..end]) {
-      var len := length(data[start..end]);
-      MulDivCancel(len, USESM.UniformSize() as nat);
-      Seq.lemma_seq_slice_slice(newdata,
-        start as nat,
-        end as nat,
-        sizeOfLengthField() as nat,
-        sizeOfLengthField() as nat + len * USESM.UniformSize() as nat);
-      Seq.lemma_seq_slice_slice(data,
-        start as nat,
-        end as nat,
-        sizeOfLengthField() as nat,
-        sizeOfLengthField() as nat + len * USESM.UniformSize() as nat);
-      var subdata := data[start + sizeOfLengthField()..start as nat + sizeOfLengthField() as nat + len * USESM.UniformSize() as nat];
-      USESM.index_bounds_facts(subdata, idx as nat);
-      Seq.lemma_seq_slice_slice(newdata, 
-        start as nat + sizeOfLengthField() as nat,
-        start as nat + sizeOfLengthField() as nat + len * USESM.UniformSize() as nat,
-        idx as nat * USESM.UniformSize() as nat,
-        (idx as nat + 1) * USESM.UniformSize() as nat);
-      USESM.setted_parsing(
-        data[start..end][sizeOfLengthField()..sizeOfLengthField() as nat + len * USESM.UniformSize() as nat],
-        idx as nat, value,
-        newdata[start..end][sizeOfLengthField()..sizeOfLengthField() as nat + len * USESM.UniformSize() as nat]);
-    }
-  }
-
-  lemma ElementDataSimplification(data: mseq<byte>, start: nat, end: nat, idx: nat)
-    requires start <= end <= |data|
-    requires sizeOfLengthField() as nat <= end - start
-    requires idx < maxLength(data[start..end])
-    ensures 0
-            <= start + sizeOfLengthField() as nat + idx * USESM.UniformSize() as nat
-            <= start + sizeOfLengthField() as nat + idx * USESM.UniformSize() as nat + USESM.UniformSize() as nat
-            <= |data|
-    ensures
-    ElementData(data[start..end], idx as uint64)
-    ==
-    data
-      [start + sizeOfLengthField() as nat + idx * USESM.UniformSize() as nat
-       ..start + sizeOfLengthField() as nat + idx * USESM.UniformSize() as nat + USESM.UniformSize() as nat]
-  {
-    PosMulPreservesOrder(idx, idx + 1, USESM.UniformSize() as nat);
-    NatMulNatIsNat(idx, USESM.UniformSize() as nat);
-    NLarith.DistributeLeft(idx, 1, USESM.UniformSize() as nat);
-    PosMulPreservesLe(idx + 1, maxLength(data[start..end]), USESM.UniformSize() as nat);
-
-    Seq.lemma_seq_slice_slice(
-      data,
-      start, end,
-      sizeOfLengthField() as nat, end - start);
-    Seq.lemma_seq_slice_slice(
-      data,
-      start + sizeOfLengthField() as nat,
-      end,
-      idx * USESM.UniformSize() as nat,
-      (idx + 1) * USESM.UniformSize() as nat);
-
-    Seq.lemma_seq_slice_slice(
-      data,
-      start, end,
-      sizeOfLengthField() as nat, sizeOfLengthField() as nat + maxLength(data[start..end]) * USESM.UniformSize() as nat);
-    Seq.lemma_seq_slice_slice(
-      data,
-      start + sizeOfLengthField() as nat,
-      start + sizeOfLengthField() as nat + maxLength(data[start..end]) * USESM.UniformSize() as nat,
-      idx * USESM.UniformSize() as nat,
-      (idx + 1) * USESM.UniformSize() as nat);
-  }
-
-  predicate resizable(data: mseq<byte>, newlen: nat) {
-    && lengthable(data)
-    && newlen <= maxLength(data)
-    && LengthInt.fitsInInteger(newlen as uint64)
-  }
-
-  method Resizable(data: mseq<byte>, newlen: uint64)
-    returns (r: bool)
-    ensures r == resizable(data, newlen as nat)
-  {
-    var l := Lengthable(data);
-    if l {
-      var maxlen := USESM.Length(data[LengthInt.Size()..]);
-      r := newlen <= maxlen && LengthInt.fitsInInteger(newlen);
-    } else {
-      r := false;
-    }
-  }
-
-  method Resize(linear data: mseq<byte>, start: uint64, end: uint64, newlen: uint64)
-    returns (linear newdata: mseq<byte>)
-    requires start as nat <= end as nat <= |data|
-    requires resizable(data[start..end], newlen as nat)
-    requires forall i | 0 <= i < newlen :: ElementMarshalling.parsable(ElementData(data[start..end], i))
-    ensures |newdata| == |data|
-    ensures forall i | 0 <= i < start :: newdata[i] == data[i]
-    ensures forall i | end as nat <= i < |newdata| :: newdata[i] == data[i]
-    ensures lengthable(newdata[start..end])
-    ensures length(newdata[start..end]) == newlen as nat
-    ensures parsable(data[start..end]) ==> parsable(newdata[start..end])
-    ensures parsable(data[start..end]) ==> |parse(newdata[start..end])| == newlen as nat
-    ensures parsable(data[start..end]) ==> Seq.agree(parse(newdata[start..end]), parse(data[start..end]))
-  {
-    var newend;
-    newdata, newend := LengthMarshalling.Marshall(LengthInt.fromUint64(newlen), data, start);
-
-    assert newdata[start..end][..LengthInt.Size()] == newdata[start..start + LengthInt.Size()];
-    LengthInt.fromtoInverses();
-
-    if parsable(data[start..end]) {
-      var len := length(data[start..end]);
-      NatMulNatIsNat(newlen as nat, USESM.UniformSize() as nat);
-      PosMulPreservesLe(newlen as nat, maxLength(data[start..end]), USESM.UniformSize() as nat);
-      Seq.lemma_seq_slice_slice(newdata,
-        start as nat,
-        end as nat,
-        sizeOfLengthField() as nat,
-        sizeOfLengthField() as nat + newlen as nat * USESM.UniformSize() as nat);
-      MulDivCancel(newlen as nat, USESM.UniformSize() as nat);
-      forall i | 0 <= i < newlen as nat
-        ensures ElementData(newdata[start..end], i as uint64) == ElementData(data[start..end], i as uint64);
-      {
-        MulDivCancel(newlen as nat, USESM.UniformSize() as nat);
-        ElementDataSimplification(data, start as nat, end as nat, i);
-        ElementDataSimplification(newdata, start as nat, end as nat, i);
-        NatMulNatIsNat(i as nat, USESM.UniformSize() as nat);
-        assert ElementData(newdata[start..end], i as uint64) == ElementData(data[start..end], i as uint64);
-      }
-
-      parsable_simplification(data[start..end]);
-      parsable_simplification(newdata[start..end]);
-
-      parse_simplification(data[start..end]);
-      parse_simplification(newdata[start..end]);
-    }
-  }
-
-  function USESMData(data: mseq<byte>) : mseq<byte>
-    requires lengthable'(data)
-  {
-    data[sizeOfLengthField()..sizeOfLengthField() as nat + length(data) * USESM.UniformSize() as nat]
-  }
-  
-  lemma ElementDataIsUSESMElementData(data: mseq<byte>, i: nat)
-    requires lengthable'(data)
-    requires i < length(data)
-    ensures USESM.length(USESMData(data)) == length(data)
-    ensures ElementData(data, i as uint64) == USESM.ElementData(USESMData(data), i as uint64)
-  {
-    var len := length(data);
-    MulDivCancel(len, USESM.UniformSize() as nat);
-    ElementDataSimplification(data, 0, |data|, i);
-    NatMulNatIsNat(i, USESM.UniformSize() as nat);
-    NLarith.DistributeLeft(i, 1, USESM.UniformSize() as nat);
-    PosMulPreservesLe(i + 1, len, USESM.UniformSize() as nat);
-    Seq.lemma_seq_slice_slice(data,
-      sizeOfLengthField() as nat, sizeOfLengthField() as nat + len * USESM.UniformSize() as nat,
-      i * USESM.UniformSize() as nat, i * USESM.UniformSize() as nat + USESM.UniformSize() as nat);
-  }
-  
-  predicate parsable(data: mseq<byte>) {
-    && lengthable'(data)
-    && var len := length(data);
-    && USESM.parsable(USESMData(data))
-  }
-
-  predicate parsable'(data: mseq<byte>) {
-    && lengthable'(data)
-    && var len := length(data);
-    && forall i | 0 <= i < len :: ElementMarshalling.parsable(ElementData(data, i as uint64))
-  }
-
-  lemma parsable_simplification(data: mseq<byte>)
-    ensures parsable(data) <==> parsable'(data)
-  {
-    if lengthable'(data) {
-      var len := length(data);
-      MulDivCancel(len, USESM.UniformSize() as nat);
-      forall i | 0 <= i < length(data)
-        ensures ElementData(data, i as uint64) == USESM.ElementData(USESMData(data), i as uint64)
-      {
-        ElementDataIsUSESMElementData(data, i);
-      }
-    }
-  }
-  
-  function parse(data: mseq<byte>) : UnmarshalledType {
-    var len := length(data);
-    USESM.parse(USESMData(data))
-  }
-
-  function parse'(data: mseq<byte>) : UnmarshalledType
-    requires parse.requires(data)
-  {
-    var len := length(data);
-    parsable_simplification(data);
-    var result: seq<Element> := seq(len, i requires 0 <= i < len => ElementMarshalling.parse(ElementData(data, i as uint64)));
-    assert |result| < Uint64UpperBound();
-    result
-  }
-
-  lemma parse_simplification(data: mseq<byte>)
-    requires parsable(data) || parsable'(data)
-    ensures parsable(data) && parsable'(data)
-    ensures parse(data) == parse'(data)
-  {
-    parsable_simplification(data);
-    parse_length(data);
-    forall i | 0 <= i < length(data)
-      ensures ElementData(data, i as uint64) == USESM.ElementData(USESMData(data), i as uint64)
-    {
-      ElementDataIsUSESMElementData(data, i);
-    }
-    assert forall i | 0 <= i < |parse(data)| :: parse(data)[i] == parse'(data)[i];
-  }
-
-  lemma parse_length(data: mseq<byte>)
-    requires parsable(data)
-    ensures |parse(data)| == length(data)
-  {
-    MulDivCancel(length(data), USESM.UniformSize() as nat);
-  }
-
-  method TryParse(data: mseq<byte>) returns (ovalue: Option<UnmarshalledType>) {
-    var olen := TryLength(data);
-    if olen == None {
-      return None;
-    }
-    ovalue := USESM.TryParse(data[sizeOfLengthField()..sizeOfLengthField() + olen.value * USESM.UniformSize()]);
-  }
-
-  method Parsable(data: mseq<byte>) returns (p: bool) {
-    var olen := TryLength(data);
-    if olen == None {
-      return false;
-    }
-    p := USESM.Parsable(data[sizeOfLengthField()..sizeOfLengthField() + olen.value * USESM.UniformSize()]);
-  }
-
-  method Parse(data: mseq<byte>) returns (value: UnmarshalledType) {
-    var len := Length(data);
-    value := USESM.Parse(data[sizeOfLengthField()..sizeOfLengthField() + len * USESM.UniformSize()]);
+    && tableable(data)
+    && var struct := partialParse(data);
+    && structGettable(struct, idx)
   }
 }
-
-// ////////////////////////////////////////////////////////
-// // Interface for appending items to marshalled sequences
-// ////////////////////////////////////////////////////////
-
-// abstract module AppendableSeqMarshalling refines SeqMarshalling {
-//   predicate appendable(data: mseq<byte>, newItemSize: nat)
-
-//   method Appendable(data: mseq<byte>, newItemSize: uint64) returns (app: bool)
-//     ensures app == appendable(data, newItemSize as nat)
-
-//   method Append(linear data: mseq<byte>, start: uint64, end: uint64, elt: Element)
-//     returns (linear newdata: mseq<byte>)
-//     requires ElementMarshalling.marshallable(elt)
-//     requires start as nat <= end as nat <= |data|
-//     requires appendable(data[start..end], ElementMarshalling.size(elt))
-//     ensures |newdata| == |data|
-//     ensures forall i | 0 <= i < start :: newdata[i] == data[i]
-//     ensures forall i | end as nat <= i < |newdata| :: newdata[i] == data[i]
-//     ensures parsable(data[start..end]) ==> parsable(newdata[start..end])
-//     ensures parsable(data[start..end]) ==> parse(newdata[start..end]) == parse(data[start..end]) + [ elt ]
-// }
-
-// //////////////////////////////////////////////////////////////////////
-// // Implementation of marshalling a general sequence of items
-// //////////////////////////////////////////////////////////////////////
-
-// abstract module VariableSizedElementSeqMarshalling refines AppendableSeqMarshalling {
-//   import LengthMarshalling : IntegerMarshalling
-//   import BoundarySeqMarshalling : IntegerSeqMarshalling
-//   import opened Sequences
-
-//   import LengthInt = LengthMarshalling.Int
-//   import BoundaryInt = BoundarySeqMarshalling.Int
-
-//   type Length = LengthMarshalling.Int.Integer
-//   type Boundary = BoundarySeqMarshalling.Int.Integer
-
-//   type BoundaryTable = mseq<Boundary>
-
-//   // INTERNAL FUNCTIONS
-
-//   function sizeOfLengthField() : nat {
-//     LengthInt.Size() as nat
-//   }
-
-//   function sizeOfBoundaryEntry() : nat {
-//     BoundaryInt.Size() as nat
-//   }
-
-//   predicate lengthable'(data: mseq<byte>)
-//   {
-//     && sizeOfLengthField() <= |data|
-//     && 0 <= LengthInt.toInt(LengthMarshalling.parse(data[..sizeOfLengthField()]))
-//   }
-
-//   function length'(data: mseq<byte>) : nat
-//     requires lengthable'(data)
-//   {
-//     LengthInt.toInt(LengthMarshalling.parse(data[..sizeOfLengthField()]))
-//   }
-
-//   datatype Structure = Structure(boundaries: mseq<Boundary>, elements: mseq<byte>)
-
-//   function sizeOfTable(len: nat) : nat {
-//     len * sizeOfBoundaryEntry()
-//   }
-
-//   predicate tableable(data: mseq<byte>) {
-//     && lengthable'(data)
-//     && var len := length'(data);
-//     && sizeOfLengthField() + sizeOfTable(len) <= |data|
-//   }
-
-//   function tabledata(data: mseq<byte>) : seq<byte>
-//     requires tableable(data)
-//   {
-//     var len := length'(data);
-//     data[sizeOfLengthField()..sizeOfLengthField() + sizeOfTable(len)]
-//   }
-
-//   function table(data: mseq<byte>) : BoundaryTable
-//     requires tableable(data)
-//   {
-//     var td := tabledata(data);
-//     BoundarySeqMarshalling.always_parsable(td);
-//     BoundarySeqMarshalling.parse(td)
-//   }
-
-//   function elementsSize(data: mseq<byte>) : nat
-//     requires tableable(data)
-//   {
-//     var tb: seq<Boundary> := table(data);
-//     if |tb| == 0 then
-//       0
-//     else if BoundaryInt.toInt(Last(tb)) < 0 then
-//       0
-//     else
-//       BoundaryInt.toInt(Last(tb))
-//   }
-
-//   predicate tableEndInBounds(data: mseq<byte>)
-//     requires tableable(data)
-//   {
-//     elementsSize(data) <= |data| - sizeOfLengthField() - sizeOfTable(length'(data))
-//   }
-
-//   function elementsData(data: mseq<byte>) : mseq<byte>
-//     requires tableable(data)
-//   {
-//     var tb := table(data);
-//     data // FIXME
-//   }
-
-//   function partialParse(data: mseq<byte>) : (result: Structure)
-//     requires tableable(data)
-//   {
-//     Structure(table(data), elementsData(data))
-//   }
-
-//   predicate structGettable(struct: Structure, idx: nat) {
-//     && idx < |struct.boundaries|
-//     && var start := BoundaryInt.toInt(struct.boundaries[idx]);
-//     && var end := if idx == 0 then |struct.elements| else BoundaryInt.toInt(struct.boundaries[idx-1]);
-//     && 0 <= start <= end <= |struct.elements|
-//   }
-
-//   function structGet(struct: Structure, idx: nat) : mseq<byte>
-//     requires structGettable(struct, idx)
-//   {
-//     var start := BoundaryInt.toInt(struct.boundaries[idx]);
-//     var end := if idx == 0 then |struct.elements| else BoundaryInt.toInt(struct.boundaries[idx-1]);
-//     struct.elements[start..end]
-//   }
-
-//   // function get(data: mseq<byte>, idx: nat) : mseq<byte>
-//   //   requires gettable(data, idx)
-//   // {
-//   //   structGet(partialParse(data), idx)
-//   // }
-
-// //   method TryGet(data: mseq<byte>, idx: uint64) returns (oedata: Option<mseq<byte>>)
-// //   {
-// //     var ostruct := PartialParse(data);
-// //     if ostruct == None || |ostruct.value.boundaries| as uint64 <= idx {
-// //       return None;
-// //     }
-// //     var struct := ostruct.value;
-
-// //     var start := BoundarySeqMarshalling.Int.toUint64(struct.boundaries[idx]);
-// //     var end := |struct.elements| as uint64;
-// //     if 0 < idx {
-// //       end := BoundarySeqMarshalling.Int.toUint64(struct.boundaries[idx]);
-// //     }
-
-// //     if start <= end <= |struct.elements| as uint64 {
-// //       oedata := Some(struct.elements[start..end]);
-// //     } else {
-// //       oedata := None;
-// //     }
-
-// //   }
-
-// //   method Gettable(data: mseq<byte>, idx: uint64) returns (g: bool)
-// //   {
-// //     var oedata := TryGet(data, idx);
-// //     return oedata.Some?;
-// //   }
-
-// //   method Get(data: mseq<byte>, idx: uint64) returns (edata: mseq<byte>)
-// //   {
-// //     var oedata := TryGet(data, idx);
-// //     return oedata.value;
-// //   }
-
-//   predicate structParsable(struct: Structure) {
-//     && (forall i | 0 <= i < |struct.boundaries| :: structGettable(struct, i))
-//     && (forall i | 0 <= i < |struct.boundaries| :: ElementMarshalling.parsable(structGet(struct, i)))
-//   }
-
-//   function structParse(struct: Structure, prefixLen: nat) : mseq<Element>
-//     requires prefixLen <= |struct.boundaries|
-//     requires structParsable(struct)
-//   {
-//     if prefixLen == 0 then
-//       []
-//     else
-//       structParse(struct, prefixLen - 1) + [ ElementMarshalling.parse(structGet(struct, prefixLen - 1)) ]
-//   }
-
-//   predicate parsable(data: mseq<byte>) {
-//     && tableable(data)
-//     && var struct := partialParse(data);
-//     && structParsable(struct)
-//   }
-
-//   function parse(data: mseq<byte>) : UnmarshalledType {
-//     var struct := partialParse(data);
-//     structParse(struct, |struct.boundaries|)
-//   }
-
-// //   method PartialParse(data: mseq<byte>) returns (oresult : Option<Structure>)
-// //     ensures oresult.Some? <==> tableable(data)
-// //     ensures tableable(data) ==> oresult.value == partialParse(data)
-// //   {
-// //     var olen := TryLength(data);
-// //     if olen == None {
-// //       return None;
-// //     }
-// //     var len := olen.value;
-
-// //     var tbdata := data[LengthMarshalling.Int.Size()..LengthMarshalling.Int.Size() + len * BoundarySeqMarshalling.Int.Size()];
-// //     var table := BoundarySeqMarshalling.Parse(tbdata);
-// //     var esdata := data[LengthMarshalling.Int.Size()..];
-// //     oresult := Some(Structure(table, esdata));
-// //   }
-
-
-// //   method TryLength(data: mseq<byte>) returns (olen: Option<uint64>)
-// //   {
-// //     if LengthMarshalling.Int.Size() <= |data| as uint64 {
-// //       var l := LengthMarshalling.Parse(data[..LengthMarshalling.Int.Size()]);
-// //       olen := Some(LengthMarshalling.Int.toUint64(l));
-// //     } else {
-// //       olen := None;
-// //     }
-// //   }
-
-// //   method Lengthable(data: mseq<byte>) returns (l: bool)
-// //   {
-// //     l := LengthMarshalling.Int.Size() <= |data| as uint64;
-// //   }
-
-// //   method Length(data: mseq<byte>) returns (len: uint64)
-// //     ensures len as nat == length(data)
-// //   {
-// //     var l := LengthMarshalling.Parse(data[..LengthMarshalling.Int.Size()]);
-// //     len := LengthMarshalling.Int.toUint64(l);
-// //   }
-
-
-// //   predicate gettable(data: mseq<byte>, idx: nat)
-// //   {
-// //     && tableable(data)
-// //     && var struct := partialParse(data);
-// //     && structGettable(struct, idx)
-// //   }
-
-// }
