lib/Base/Slice.i.dfy
@@ -1,0 +1,51 @@
+include "../Lang/NativeTypes.s.dfy"
+include "../Base/sequences.i.dfy"
+
+module Slices {
+  import opened NativeTypes
+  import Seq = Sequences
+
+  datatype Slice = Slice(start: uint64, end: uint64) {
+    predicate WF() {
+      && start as nat <= end as nat
+    }
+
+    predicate WF'<T>(data': seq<T>) {
+      && start as nat <= end as nat <= |data'|
+    }
+
+    function method I<T>(data: mseq<T>) : mseq<T>
+      requires WF'(data)
+    {
+      data[start..end]
+    }
+
+    function method sub(a: uint64, b: uint64) : (result: Slice)
+      requires WF()
+      requires a <= b <= end - start
+      ensures result.WF()
+    {
+      Slice(start + a, start + b)
+    }
+  }
+
+  function method operator(| |)(slice: Slice) : (result: uint64)
+    requires slice.WF()
+  {
+    slice.end - slice.start
+  }
+
+  function method all(data: mseq) : (result: Slice)
+    ensures all(data).WF'(data)
+    ensures all(data).I(data) == data
+  {
+    Slice(0, |data| as uint64)
+  }
+
+  predicate subSlice(smaller: Slice, superSlice: Slice)
+    requires smaller.WF()
+    requires superSlice.WF()
+  {
+    && superSlice.start <= smaller.start <= smaller.end <= superSlice.end
+  }
+}
