lib/Marshalling/NLarith.i.dfy
@@ -1,4 +1,8 @@
+include "../Lang/NativeTypes.s.dfy"
+
 module NLarith {
+  import opened NativeTypes
+
   lemma DivLe(a: nat, b: nat)
     requires 0 < b
     ensures 0 <= a / b <= a
@@ -14,6 +18,13 @@ module NLarith {
   lemma DistributeLeft(a: int, b: int, c: int)
     ensures (a + b) * c == a * c + b * c
   {
+  }
+
+  method Uint64Mult(a: uint64, b: uint64) returns (c: uint64)
+    requires a as nat * b as nat < Uint64UpperBound()
+    ensures c as nat == a as nat * b as nat
+  {
+    c := a * b;
   }
 }
   
